upd(wip): rename Universe to UnivLvl, family to Sort and Sort to Universe

common/theories/Universes.v
@@ -1,7 +1,7 @@
 From Stdlib Require Import OrdersAlt MSetList MSetAVL MSetFacts MSetProperties MSetDecide FMapAVL.
 From Equations Require Import Equations.
 From MetaRocq.Utils Require Import utils MRMSets MRFSets.
-From MetaRocq.Common Require Import BasicAst config.
+From MetaRocq.Common Require Import BasicAst config Levels Sorts.
 From Stdlib Require Import ssreflect.
 
 Local Open Scope nat_scope.
@@ -9,1627 +9,180 @@ Local Open Scope string_scope2.
 
 Implicit Types (cf : checker_flags).
 
-Ltac absurd :=
-  match goal with
-  | [H: ~ True |- _] => elim (H I)
-  | [H : False |- _] => elim H
-  | H: is_true false |- _ => discriminate H
-  | |- False -> _ => let H := fresh in intro H; elim H
-  | |- _ -> False -> _ => let H := fresh in intros ? H; elim H
-  | |- is_true false -> _ => let H := fresh in intro H; discriminate H
-  | |- _ -> is_true false -> _ => let H := fresh in intros ? H; discriminate H
-  end.
-#[global]
-Hint Extern 10 => absurd : core.
-
-(** * Valuations *)
-
-(** A valuation is a universe level (nat) given for each
-    universe lvariable (Level.t).
-    It is >= for polymorphic concrete_sort and > 0 for monomorphic concrete_sort. *)
-Record valuation :=
-  { valuation_mono : string -> positive ;
-    valuation_poly : nat -> nat }.
-
-Class Evaluable (A : Type) := val : valuation -> A -> nat.
-
-
-(** Levels are Set or Level or lvar *)
-Module Level.
-  Inductive t_ : Set :=
-  | lzero
-  | level (_ : string)
-  | lvar (_ : nat) (* these are debruijn indices *).
-  Derive NoConfusion for t_.
-
-  Definition t := t_.
-
-  Definition is_set (x : t) :=
-    match x with
-    | lzero => true
-    | _ => false
-    end.
-
-  Definition is_var (l : t) :=
-    match l with
-    | lvar _ => true
-    | _ => false
-    end.
-
-  Global Instance Evaluable : Evaluable t
-    := fun v l => match l with
-               | lzero =>  (0%nat)
-               | level s => (Pos.to_nat (v.(valuation_mono) s))
-               | lvar x => (v.(valuation_poly) x)
-               end.
-
-
-  Definition compare (l1 l2 : t) : comparison :=
-    match l1, l2 with
-    | lzero, lzero => Eq
-    | lzero, _ => Lt
-    | _, lzero => Gt
-    | level s1, level s2 => string_compare s1 s2
-    | level _, _ => Lt
-    | _, level _ => Gt
-    | lvar n, lvar m => Nat.compare n m
-    end.
-
-  Definition eq : t -> t -> Prop := eq.
-  Definition eq_equiv : Equivalence eq := _.
-
-  Inductive lt_ : t -> t -> Prop :=
-  | ltSetLevel s : lt_ lzero (level s)
-  | ltSetlvar n : lt_ lzero (lvar n)
-  | ltLevelLevel s s' : StringOT.lt s s' -> lt_ (level s) (level s')
-  | ltLevellvar s n : lt_ (level s) (lvar n)
-  | ltlvarlvar n n' : Nat.lt n n' -> lt_ (lvar n) (lvar n').
-  Derive Signature for lt_.
-
-  Definition lt := lt_.
-
-  Definition lt_strorder : StrictOrder lt.
-  Proof.
-    constructor.
-    - intros [| |] X; inversion X.
-      now eapply irreflexivity in H1.
-      eapply Nat.lt_irrefl; tea.
-    - intros [| |] [| |] [| |] X1 X2;
-        inversion X1; inversion X2; constructor.
-      now transitivity s0.
-      etransitivity; tea.
-  Qed.
-
-  Definition lt_compat : Proper (eq ==> eq ==> iff) lt.
-  Proof.
-    intros x y e z t e'. unfold eq in *; subst. reflexivity.
-  Qed.
-
-  Definition compare_spec :
-    forall x y : t, CompareSpec (x = y) (lt x y) (lt y x) (compare x y).
-  Proof.
-    intros [] []; repeat constructor.
-    - eapply CompareSpec_Proper.
-      5: eapply CompareSpec_string. 4: reflexivity.
-      all: split; [now inversion 1|]. now intros ->.
-      all: intro; now constructor.
-    - eapply CompareSpec_Proper.
-      5: eapply Nat.compare_spec. 4: reflexivity.
-      all: split; [now inversion 1|]. now intros ->.
-      all: intro; now constructor.
-  Qed.
-
-  Definition eq_level l1 l2 :=
-    match l1, l2 with
-    | Level.lzero, Level.lzero => true
-    | Level.level     s1, Level.level     s2 => ReflectEq.eqb s1 s2
-    | Level.lvar n1, Level.lvar n2 => ReflectEq.eqb n1 n2
-    | _, _ => false
-    end.
-
-  #[global, program] Instance reflect_level : ReflectEq Level.t := {
-    eqb := eq_level
-  }.
-  Next Obligation.
-    destruct x, y.
-    all: unfold eq_level.
-    all: try solve [ constructor ; reflexivity ].
-    all: try solve [ constructor ; discriminate ].
-    - destruct (ReflectEq.eqb_spec t0 t1) ; nodec.
-      constructor. f_equal. assumption.
-    - destruct (ReflectEq.eqb_spec n n0) ; nodec.
-      constructor. subst. reflexivity.
-  Defined.
-
-  Global Instance eqb_refl : @Reflexive Level.t eqb.
-  Proof.
-    intros x. apply ReflectEq.eqb_refl.
-  Qed.
-
-  Definition eqb := eq_level.
-
-  Lemma eqb_spec l l' : reflect (eq l l') (eqb l l').
-  Proof.
-    apply reflectProp_reflect.
-    now generalize (eqb_spec l l').
-  Qed.
-
-  Definition eq_leibniz (x y : t) : eq x y -> x = y := id.
-
-  Definition eq_dec : forall (l1 l2 : t), {l1 = l2}+{l1 <> l2} := Classes.eq_dec.
-
-End Level.
-
-Module LevelSet := MSetAVL.Make Level.
-Module LevelSetFact := WFactsOn Level LevelSet.
-Module LevelSetOrdProp := MSetProperties.OrdProperties LevelSet.
-Module LevelSetProp := LevelSetOrdProp.P.
-Module LevelSetDecide := LevelSetProp.Dec.
-Module LevelSetExtraOrdProp := MSets.ExtraOrdProperties LevelSet LevelSetOrdProp.
-Module LevelSetExtraDecide := MSetAVL.Decide Level LevelSet.
-Module LS := LevelSet.
-
-Ltac lsets := LevelSetDecide.fsetdec.
-Notation "(=_lset)" := LevelSet.Equal (at level 0).
-Infix "=_lset" := LevelSet.Equal (at level 30).
-Notation "(==_lset)" := LevelSet.equal (at level 0).
-Infix "==_lset" := LevelSet.equal (at level 30).
-
-Section LevelSetMoreFacts.
-
-  Definition LevelSet_pair x y
-    := LevelSet.add y (LevelSet.singleton x).
-
-  Lemma LevelSet_pair_In x y z :
-    LevelSet.In x (LevelSet_pair y z) -> x = y \/ x = z.
-  Proof.
-    intro H. apply LevelSetFact.add_iff in H.
-    destruct H; [intuition|].
-    apply LevelSetFact.singleton_1 in H; intuition.
-  Qed.
-
-  Definition LevelSet_mem_union (s s' : LevelSet.t) x :
-    LevelSet.mem x (LevelSet.union s s') <-> LevelSet.mem x s \/ LevelSet.mem x s'.
-  Proof.
-    rewrite LevelSetFact.union_b.
-    apply orb_true_iff.
-  Qed.
-
-  Lemma LevelSet_In_fold_right_add x l :
-    In x l <-> LevelSet.In x (fold_right LevelSet.add LevelSet.empty l).
-  Proof.
-    split.
-    - induction l; simpl => //.
-      intros [<-|H].
-      * eapply LevelSet.add_spec; left; auto.
-      * eapply LevelSet.add_spec; right; auto.
-    - induction l; simpl => //.
-      * now rewrite LevelSetFact.empty_iff.
-      * rewrite LevelSet.add_spec. intuition auto.
-  Qed.
-
-  Lemma LevelSet_union_empty s : LevelSet.Equal (LevelSet.union LevelSet.empty s) s.
-  Proof.
-    intros x; rewrite LevelSet.union_spec. lsets.
-  Qed.
-End LevelSetMoreFacts.
-
-(* prop level is Prop or SProp *)
-Module PropLevel.
-
-  Inductive t := lSProp | lProp.
-  Derive NoConfusion EqDec for t.
-  (* Global Instance PropLevel_Evaluable : Evaluable t :=
-    fun v l => match l with
-              lSProp => -1
-            | lProp => -1
-            end. *)
-
-  Definition compare (l1 l2 : t) : comparison :=
-    match l1, l2 with
-    | lSProp, lSProp  => Eq
-    | lProp, lProp  => Eq
-    | lProp, lSProp => Gt
-    | lSProp, lProp => Lt
-    end.
-
-  Inductive lt_ : t -> t -> Prop :=
-    ltSPropProp : lt_ lSProp lProp.
-
-  Definition lt := lt_.
-
-  Global Instance lt_strorder : StrictOrder lt.
-  split.
-  - intros n X. destruct n;inversion X.
-  - intros n1 n2 n3 X1 X2. destruct n1,n2,n3;auto; try inversion X1;try inversion X2.
-  Defined.
-
-End PropLevel.
-
-Module LevelExpr.
-  Definition t := (Level.t * nat)%type.
-
-  Global Instance Evaluable : Evaluable t
-    := fun v l => (snd l + val v (fst l)).
-
-  Definition succ (l : t) := (fst l, S (snd l)).
-
-  Definition get_level (e : t) : Level.t := fst e.
-
-  Definition get_noprop (e : LevelExpr.t) := Some (fst e).
-
-  Definition is_level (e : t) : bool :=
-    match e with
-    | (_, 0%nat) => true
-    | _  => false
-    end.
-
-  Definition make (l : Level.t) : t := (l, 0%nat).
-
-  Definition set : t := (Level.lzero, 0%nat).
-  Definition type1 : t := (Level.lzero, 1%nat).
-
-  Definition eq : t -> t -> Prop := eq.
-
-  Definition eq_equiv : Equivalence eq := _.
-
-  Inductive lt_ : t -> t -> Prop :=
-  | ltLevelExpr1 l n n' : (n < n')%nat -> lt_ (l, n) (l, n')
-  | ltLevelExpr2 l l' b b' : Level.lt l l' -> lt_ (l, b) (l', b').
-
-  Definition lt := lt_.
-
-  Global Instance lt_strorder : StrictOrder lt.
-  Proof.
-    constructor.
-    - intros x X; inversion X. subst. lia. subst.
-      eapply Level.lt_strorder; eassumption.
-    - intros x y z X1 X2; invs X1; invs X2; constructor; tea.
-      etransitivity; tea.
-      etransitivity; tea.
-  Qed.
-
-  Definition lt_compat : Proper (Logic.eq ==> Logic.eq ==> iff) lt.
-    intros x x' H1 y y' H2; now rewrite H1 H2.
-  Qed.
-
-  Definition compare (x y : t) : comparison :=
-    match x, y with
-    | (l1, b1), (l2, b2) =>
-      match Level.compare l1 l2 with
-      | Eq => Nat.compare b1 b2
-      | x => x
-      end
-    end.
-
-  Definition compare_spec :
-    forall x y : t, CompareSpec (x = y) (lt x y) (lt y x) (compare x y).
-  Proof.
-    intros [? ?] [? ?]; cbn; repeat constructor.
-    destruct (Level.compare_spec t0 t1); repeat constructor; tas.
-    subst.
-    destruct (Nat.compare_spec n n0); repeat constructor; tas. congruence.
-  Qed.
-
-  Global Instance reflect_t : ReflectEq t := reflect_prod _ _ .
-
-  Definition eq_dec : forall (l1 l2 : t), {l1 = l2} + {l1 <> l2} := Classes.eq_dec.
-
-  Definition eq_leibniz (x y : t) : eq x y -> x = y := id.
-
-  Lemma val_make v l
-    : val v (LevelExpr.make l) = val v l.
-  Proof.
-    destruct l eqn:H; cbnr.
-  Qed.
-
-  Lemma val_make_npl v (l : Level.t)
-    : val v (LevelExpr.make l) = val v l.
-  Proof.
-    destruct l; cbnr.
-  Qed.
-
-End LevelExpr.
-
-Module LevelExprSet := MSetList.MakeWithLeibniz LevelExpr.
-Module LevelExprSetFact := WFactsOn LevelExpr LevelExprSet.
-Module LevelExprSetOrdProp := MSetProperties.OrdProperties LevelExprSet.
-Module LevelExprSetProp := LevelExprSetOrdProp.P.
-Module LevelExprSetDecide := LevelExprSetProp.Dec.
-Module LevelExprSetExtraOrdProp := MSets.ExtraOrdProperties LevelExprSet LevelExprSetOrdProp.
-
-(* We have decidable equality w.r.t leibniz equality for sets of levels.
-  This means concrete_sort also has a decidable equality. *)
-#[global, program] Instance levelexprset_reflect : ReflectEq LevelExprSet.t :=
-  { eqb := LevelExprSet.equal }.
-Next Obligation.
-  destruct (LevelExprSet.equal x y) eqn:e; constructor.
-  eapply LevelExprSet.equal_spec in e.
-  now eapply LevelExprSet.eq_leibniz.
-  intros e'.
-  subst y.
-  pose proof (@LevelExprSetFact.equal_1 x x).
-  forward H. reflexivity. congruence.
-Qed.
-
-#[global] Instance levelexprset_eq_dec : Classes.EqDec LevelExprSet.t := Classes.eq_dec.
-
-
-
-Record nonEmptyLevelExprSet
-  := { t_set : LevelExprSet.t ;
-       t_ne  : LevelExprSet.is_empty t_set = false }.
-
-Derive NoConfusion for nonEmptyLevelExprSet.
-
-(** This coercion allows to see the non-empty set as a regular [LevelExprSet.t] *)
-Coercion t_set : nonEmptyLevelExprSet >-> LevelExprSet.t.
-
-Module NonEmptySetFacts.
-  Definition singleton (e : LevelExpr.t) : nonEmptyLevelExprSet
-    := {| t_set := LevelExprSet.singleton e;
-          t_ne := eq_refl |}.
-
-  Lemma not_Empty_is_empty s :
-    ~ LevelExprSet.Empty s -> LevelExprSet.is_empty s = false.
-  Proof.
-    intro H. apply not_true_is_false. intro H'.
-    apply H. now apply LevelExprSetFact.is_empty_2 in H'.
-  Qed.
-
-  Program Definition add (e : LevelExpr.t) (u : nonEmptyLevelExprSet) : nonEmptyLevelExprSet
-    := {| t_set := LevelExprSet.add e u |}.
-  Next Obligation.
-    apply not_Empty_is_empty; intro H.
-    eapply H. eapply LevelExprSet.add_spec.
-    left; reflexivity.
-  Qed.
-
-  Lemma add_spec e u e' :
-    LevelExprSet.In e' (add e u) <-> e' = e \/ LevelExprSet.In e' u.
-  Proof.
-    apply LevelExprSet.add_spec.
-  Qed.
-
-  Definition add_list : list LevelExpr.t -> nonEmptyLevelExprSet -> nonEmptyLevelExprSet
-    := List.fold_left (fun u e => add e u).
-
-  Lemma add_list_spec l u e :
-    LevelExprSet.In e (add_list l u) <-> In e l \/ LevelExprSet.In e u.
-  Proof.
-    unfold add_list. rewrite <- fold_left_rev_right.
-    etransitivity. 2:{ eapply or_iff_compat_r. etransitivity.
-                       2: apply @InA_In_eq with (A:=LevelExpr.t).
-                       eapply InA_rev. }
-    induction (List.rev l); cbn.
-    - split. intuition. intros [H|H]; tas. invs H.
-    - split.
-      + intro H. apply add_spec in H. destruct H as [H|H].
-        * left. now constructor.
-        * apply IHl0 in H. destruct H as [H|H]; [left|now right].
-          now constructor 2.
-      + intros [H|H]. inv H.
-        * apply add_spec; now left.
-        * apply add_spec; right. apply IHl0. now left.
-        * apply add_spec; right. apply IHl0. now right.
-  Qed.
-
-  Program Definition to_nonempty_list (u : nonEmptyLevelExprSet) : LevelExpr.t * list LevelExpr.t
-    := match LevelExprSet.elements u with
-       | [] => False_rect _ _
-       | e :: l => (e, l)
-       end.
-  Next Obligation.
-    destruct u as [u1 u2]; cbn in *. revert u2.
-    apply eq_true_false_abs.
-    unfold LevelExprSet.is_empty, LevelExprSet.Raw.is_empty,
-    LevelExprSet.elements, LevelExprSet.Raw.elements in *.
-    rewrite <- Heq_anonymous; reflexivity.
-  Qed.
-
-  Lemma singleton_to_nonempty_list e : to_nonempty_list (singleton e) = (e, []).
-  Proof. reflexivity. Defined.
-
-  Lemma to_nonempty_list_spec u :
-    let '(e, u') := to_nonempty_list u in
-    e :: u' = LevelExprSet.elements u.
-  Proof.
-    destruct u as [u1 u2].
-    unfold to_nonempty_list; cbn.
-    set (l := LevelExprSet.elements u1). unfold l at 2 3 4.
-    set (e := (eq_refl: l = LevelExprSet.elements u1)); clearbody e.
-    destruct l.
-    - exfalso. revert u2. apply eq_true_false_abs.
-      unfold LevelExprSet.is_empty, LevelExprSet.Raw.is_empty,
-      LevelExprSet.elements, LevelExprSet.Raw.elements in *.
-      rewrite <- e; reflexivity.
-    - reflexivity.
-  Qed.
-
-  Lemma to_nonempty_list_spec' u :
-    (to_nonempty_list u).1 :: (to_nonempty_list u).2 = LevelExprSet.elements u.
-  Proof.
-    pose proof (to_nonempty_list_spec u).
-    now destruct (to_nonempty_list u).
-  Qed.
-
-  Lemma In_to_nonempty_list (u : nonEmptyLevelExprSet) (e : LevelExpr.t) :
-    LevelExprSet.In e u
-    <-> e = (to_nonempty_list u).1 \/ In e (to_nonempty_list u).2.
-  Proof.
-    etransitivity. symmetry. apply LevelExprSet.elements_spec1.
-    pose proof (to_nonempty_list_spec' u) as H.
-    destruct (to_nonempty_list u) as [e' l]; cbn in *.
-    rewrite <- H; clear. etransitivity. apply InA_cons.
-    eapply or_iff_compat_l. apply InA_In_eq.
-  Qed.
-
-  Lemma In_to_nonempty_list_rev (u : nonEmptyLevelExprSet) (e : LevelExpr.t) :
-    LevelExprSet.In e u
-    <-> e = (to_nonempty_list u).1 \/ In e (List.rev (to_nonempty_list u).2).
-  Proof.
-    etransitivity. eapply In_to_nonempty_list.
-    apply or_iff_compat_l. apply in_rev.
-  Qed.
-
-  Definition map (f : LevelExpr.t -> LevelExpr.t) (u : nonEmptyLevelExprSet) : nonEmptyLevelExprSet :=
-    let '(e, l) := to_nonempty_list u in
-    add_list (List.map f l) (singleton (f e)).
-
-  Lemma map_spec f u e :
-    LevelExprSet.In e (map f u) <-> exists e0, LevelExprSet.In e0 u /\ e = (f e0).
-  Proof.
-    unfold map. symmetry. etransitivity.
-    { eapply iff_ex; intro. eapply and_iff_compat_r. eapply In_to_nonempty_list. }
-    destruct (to_nonempty_list u) as [e' l]; cbn in *.
-    symmetry. etransitivity. eapply add_list_spec.
-    etransitivity. eapply or_iff_compat_l. apply LevelExprSet.singleton_spec.
-    etransitivity. eapply or_iff_compat_r.
-    apply in_map_iff. clear u. split.
-    - intros [[e0 []]|H].
-      + exists e0. split. right; tas. congruence.
-      + exists e'. split; tas. left; reflexivity.
-    - intros [xx [[H|H] ?]].
-      + right. congruence.
-      + left. exists xx. split; tas; congruence.
-  Qed.
-
-  Program Definition non_empty_union (u v : nonEmptyLevelExprSet) : nonEmptyLevelExprSet :=
-    {| t_set := LevelExprSet.union u v |}.
-  Next Obligation.
-    apply not_Empty_is_empty; intro H.
-    assert (HH: LevelExprSet.Empty u). {
-      intros x Hx. apply (H x).
-      eapply LevelExprSet.union_spec. now left. }
-    apply LevelExprSetFact.is_empty_1 in HH.
-    rewrite t_ne in HH; discriminate.
-  Qed.
-
-  Lemma elements_not_empty (u : nonEmptyLevelExprSet) : LevelExprSet.elements u <> [].
-  Proof.
-    destruct u as [u1 u2]; cbn; intro e.
-    unfold LevelExprSet.is_empty, LevelExprSet.elements,
-    LevelExprSet.Raw.elements in *.
-    rewrite e in u2; discriminate.
-  Qed.
-
-
-  Lemma eq_univ (u v : nonEmptyLevelExprSet) :
-    u = v :> LevelExprSet.t -> u = v.
-  Proof.
-    destruct u as [u1 u2], v as [v1 v2]; cbn. intros X; destruct X.
-    now rewrite (uip_bool _ _ u2 v2).
-  Qed.
-
-  Lemma eq_univ' (u v : nonEmptyLevelExprSet) :
-    LevelExprSet.Equal u v -> u = v.
-  Proof.
-    intro H. now apply eq_univ, LevelExprSet.eq_leibniz.
-  Qed.
-
-  Lemma eq_univ'' (u v : nonEmptyLevelExprSet) :
-    LevelExprSet.elements u = LevelExprSet.elements v -> u = v.
-  Proof.
-    intro H. apply eq_univ.
-    destruct u as [u1 u2], v as [v1 v2]; cbn in *; clear u2 v2.
-    destruct u1 as [u1 u2], v1 as [v1 v2]; cbn in *.
-    destruct H. now rewrite (uip_bool _ _ u2 v2).
-  Qed.
-
-  Lemma univ_expr_eqb_true_iff (u v : nonEmptyLevelExprSet) :
-    LevelExprSet.equal u v <-> u = v.
-  Proof.
-    split.
-    - intros.
-      apply eq_univ'. now apply LevelExprSet.equal_spec.
-    - intros ->. now apply LevelExprSet.equal_spec.
-  Qed.
-
-  Lemma univ_expr_eqb_comm (u v : nonEmptyLevelExprSet) :
-    LevelExprSet.equal u v <-> LevelExprSet.equal v u.
-  Proof.
-    transitivity (u = v). 2: transitivity (v = u).
-    - apply univ_expr_eqb_true_iff.
-    - split; apply eq_sym.
-    - split; apply univ_expr_eqb_true_iff.
-  Qed.
-
-
-  Lemma LevelExprSet_for_all_false f u :
-    LevelExprSet.for_all f u = false -> LevelExprSet.exists_ (negb ∘ f) u.
-  Proof.
-    intro H. rewrite LevelExprSetFact.exists_b.
-    rewrite LevelExprSetFact.for_all_b in H.
-    all: try now intros x y [].
-    induction (LevelExprSet.elements u); cbn in *; [discriminate|].
-    apply andb_false_iff in H; apply orb_true_iff; destruct H as [H|H].
-    left; now rewrite H.
-    right; now rewrite IHl.
-  Qed.
-
-  Lemma LevelExprSet_For_all_exprs (P : LevelExpr.t -> Prop) (u : nonEmptyLevelExprSet)
-    : LevelExprSet.For_all P u
-      <-> P (to_nonempty_list u).1 /\ Forall P (to_nonempty_list u).2.
-  Proof.
-    etransitivity.
-    - eapply iff_forall; intro e. eapply imp_iff_compat_r.
-      apply In_to_nonempty_list.
-    - cbn; split.
-      + intro H. split. apply H. now left.
-        apply Forall_forall. intros x H0.  apply H; now right.
-      + intros [H1 H2] e [He|He]. subst e; tas.
-        eapply Forall_forall in H2; tea.
-  Qed.
-
-
-End NonEmptySetFacts.
-Import NonEmptySetFacts.
-
-
 Module Universe.
-  (** A universe / an algebraic expression is a list of universe expressions which is:
-        - sorted
-        - without duplicate
-        - non empty *)
+  (** A Universe is a product of a sort with a universe level.
 
-  Definition t := nonEmptyLevelExprSet.
+  	  Universes are quotiented at conversion so that every impredicative sorts (e.g., [sSProp] or [sProp])
+	  at level i and j are convertible. *)
+  Record t_ {sort} {ulvl} :=
+    mk
+	{ s : sort
+  	; l : ulvl }.
+  Arguments t_ : clear implicits.
+  Arguments mk {_ _} _ _.
 
-  (* We use uip on the is_empty condition *)
-  #[global, program] Instance levelexprset_reflect : ReflectEq t :=
-    { eqb x y := eqb x.(t_set) y.(t_set) }.
+  Definition eq_ {sort} {ulvl} eq_sort eq_ulvl (u u' : t_ sort ulvl) :=
+    eq_sort (u.(s)) (u'.(s)) /\ eq_ulvl (u.(l)) (u'.(l)).
+
+  Definition t := t_ Sort.t UnivLvl.t.
+
+  Lemma univ_eq :
+    forall (u u' : t),
+	  u.(s) = u'.(s) ->
+	  u.(l) = u'.(l) ->
+	  u = u'.
+  Proof. intros [] []; cbn in *; now intros -> ->. Qed.
+
+  Definition eqb {sort} {univ} `{ReflectEq sort} `{ReflectEq univ} (u1 u2 : t_ sort univ) : bool :=
+    eqb u1.(s) u2.(s) &&
+	eqb u1.(l) u2.(l).
+
+  #[global, program] Instance reflect_eq_univ_ {sort} {ulvl} `{ReflectEq sort} `{ReflectEq ulvl} : ReflectEq (t_ sort ulvl) :=
+    { eqb := eqb }.
   Next Obligation.
-    destruct (eqb_spec (t_set x) (t_set y)); constructor.
-    destruct x, y; cbn in *. subst.
-    now rewrite (uip t_ne0 t_ne1).
-    intros e; subst x; apply H.
-    reflexivity.
+    destruct x as [s l], y as [s' l']; unfold eqb; cbn.
+	destruct (eqb_spec s s'); destruct (eqb_spec l l').
+	all: cbn; constructor; easy.
   Qed.
 
-  #[global] Instance eq_dec_univ0 : EqDec t := eq_dec.
+  #[global] Instance eq_dec_univ {sort} {ulvl} `{EqDec sort} `{EqDec ulvl} : EqDec (t_ sort ulvl) :=
+    ltac:(intros s s'; decide equality).
 
-  Definition make (e: LevelExpr.t) : t := singleton e.
-  Definition make' (l: Level.t) : t := singleton (LevelExpr.make l).
+  Definition map {sort sort'} {ulvl ulvl'} (fs : sort -> sort') (fl : ulvl -> ulvl') u :=
+    mk (fs u.(s)) (fl u.(l)).
 
-  Lemma make'_inj l l' : make' l = make' l' -> l = l'.
-  Proof.
-    destruct l, l' => //=; now inversion 1.
-  Qed.
+  Definition maps {sort sort'} {ulvl} (f : sort -> sort') u :=
+    map f (fun (x : ulvl) => x) u.
 
-  (** The non empty / sorted / without dup list of univ expressions, the
-    components of the pair are the head and the tail of the (non empty) list *)
-  Definition exprs : t -> LevelExpr.t * list LevelExpr.t := to_nonempty_list.
+  Definition mapl {sort} {ulvl ulvl'} (f : ulvl -> ulvl') u :=
+    map (fun (x : sort) => x) f u.
 
-  Global Instance Evaluable : Evaluable Universe.t
-    := fun v u =>
-      let '(e, u) := Universe.exprs u in
-      List.fold_left (fun n e => Nat.max (val v e) n) u (val v e).
+  Definition on_sort {ulvl} {T} (P: ulvl -> T) (def: T) (u : t_ Sort.t ulvl) :=
+    match u.(s) with
+    | sProp | sSProp => def
+    | sType => P u.(l)
+    end.
 
   (** Test if the universe is a lub of levels or contains +n's. *)
   Definition is_levels (u : t) : bool :=
-    LevelExprSet.for_all LevelExpr.is_level u.
+    match u.(s) with
+    | sSProp | sProp => true
+    | sType => UnivLvl.is_levels u.(l)
+    end.
 
   (** Test if the universe is a level or an algebraic universe. *)
   Definition is_level (u : t) : bool :=
-    (LevelExprSet.cardinal u =? 1)%nat && is_levels u.
-
-  (* Used for quoting. *)
-  Definition from_kernel_repr (e : Level.t * nat) (es : list (Level.t * nat)) : t
-    := add_list es (Universe.make e).
-
-  Definition succ : t -> t := map LevelExpr.succ.
-
-  (** The l.u.b. of 2 non-prop universe sets *)
-  Definition sup : t -> t -> t := non_empty_union.
-
-  Definition get_is_level (u : t) : option Level.t :=
-    match LevelExprSet.elements u with
-    | [(l, 0%nat)] => Some l
-    | _ => None
-    end.
-
-  Lemma val_make v e : val v (make e) = val v e.
-  Proof. reflexivity. Qed.
-
-  Lemma val_make' v l
-    : val v (make' l) = val v l.
-  Proof. reflexivity. Qed.
-
-  Definition lt : t -> t -> Prop := LevelExprSet.lt.
-  Definition lt_compat : Proper (eq ==> eq ==> iff) lt.
-  Proof. repeat intro; subst; reflexivity. Qed.
-  #[global] Instance lt_strorder : StrictOrder lt.
-  Proof.
-    cbv [lt]; constructor.
-    { intros ? H. apply irreflexivity in H; assumption. }
-    { intros ??? H1 H2; etransitivity; tea. }
-  Qed.
-End Universe.
-
-Ltac u :=
-  change LevelSet.elt with Level.t in *;
-  change LevelExprSet.elt with LevelExpr.t in *.
-  (* change ConstraintSet.elt with UnivConstraint.t in *. *)
-
-
-Lemma val_fold_right (u : Universe.t) v :
-  val v u = fold_right (fun e x => Nat.max (val v e) x) (val v (Universe.exprs u).1)
-                       (List.rev (Universe.exprs u).2).
-Proof.
-  unfold val at 1, Universe.Evaluable.
-  destruct (Universe.exprs u).
-  now rewrite fold_left_rev_right.
-Qed.
-
-Lemma val_In_le (u : Universe.t) v e :
-  LevelExprSet.In e u -> val v e <= val v u.
-Proof.
-  intro H. rewrite val_fold_right.
-  apply In_to_nonempty_list_rev in H.
-  fold Universe.exprs in H; destruct (Universe.exprs u); cbn in *.
-  destruct H as [H|H].
-  - subst. induction (List.rev l); cbnr. lia.
-  - induction (List.rev l); cbn; invs H.
-    + u; lia.
-    + specialize (IHl0 H0). lia.
-Qed.
-
-Lemma val_In_max (u : Universe.t) v :
-  exists e, LevelExprSet.In e u /\ val v e = val v u.
-Proof.
-  eapply iff_ex. {
-    intro. eapply and_iff_compat_r. apply In_to_nonempty_list_rev. }
-  rewrite val_fold_right. fold Universe.exprs; destruct (Universe.exprs u) as [e l]; cbn in *.
-  clear. induction (List.rev l); cbn.
-  - exists e. split; cbnr. left; reflexivity.
-  - destruct IHl0 as [e' [H1 H2]].
-    destruct (Nat.max_dec (val v a) (fold_right (fun e0 x0 => Nat.max (val v e0) x0)
-                                               (val v e) l0)) as [H|H];
-      rewrite H; clear H.
-    + exists a. split; cbnr. right. now constructor.
-    + rewrite <- H2. exists e'. split; cbnr.
-      destruct H1 as [H1|H1]; [now left|right]. now constructor 2.
-Qed.
-
-Lemma val_ge_caract (u : Universe.t) v k :
-  (forall e, LevelExprSet.In e u -> val v e <= k) <-> val v u <= k.
-Proof.
-  split.
-  - eapply imp_iff_compat_r. {
-      eapply iff_forall; intro. eapply imp_iff_compat_r.
-      apply In_to_nonempty_list_rev. }
-    rewrite val_fold_right.
-    fold Universe.exprs; destruct (Universe.exprs u) as [e l]; cbn; clear.
-    induction (List.rev l); cbn.
-    + intros H. apply H. left; reflexivity.
-    + intros H.
-      destruct (Nat.max_dec (val v a) (fold_right (fun e0 x => Nat.max (val v e0) x)
-                                                 (val v e) l0)) as [H'|H'];
-        rewrite H'; clear H'.
-      * apply H. right. now constructor.
-      * apply IHl0. intros x [H0|H0]; apply H. now left.
-        right; now constructor 2.
-  - intros H e He. eapply val_In_le in He. etransitivity; eassumption.
-Qed.
-
-Lemma val_le_caract (u : Universe.t) v k :
-  (exists e, LevelExprSet.In e u /\ k <= val v e) <-> k <= val v u.
-Proof.
-  split.
-  - eapply imp_iff_compat_r. {
-      eapply iff_ex; intro. eapply and_iff_compat_r. apply In_to_nonempty_list_rev. }
-    rewrite val_fold_right.
-    fold Universe.exprs; destruct (Universe.exprs u) as [e l]; cbn; clear.
-    induction (List.rev l); cbn.
-    + intros H. destruct H as [e' [[H1|H1] H2]].
-      * now subst.
-      * invs H1.
-    + intros [e' [[H1|H1] H2]].
-      * forward IHl0; [|lia]. exists e'. split; tas. left; assumption.
-      * invs H1.
-        -- u; lia.
-        -- forward IHl0; [|lia]. exists e'. split; tas. right; assumption.
-  - intros H. destruct (val_In_max u v) as [e [H1 H2]].
-    exists e. rewrite H2; split; assumption.
-Qed.
-
-
-
-Lemma val_caract (u : Universe.t) v k :
-  val v u = k
-  <-> (forall e, LevelExprSet.In e u -> val v e <= k)
-    /\ exists e, LevelExprSet.In e u /\ val v e = k.
-Proof.
-  split.
-  - intros <-; split.
-    + apply val_In_le.
-    + apply val_In_max.
-  - intros [H1 H2].
-    apply val_ge_caract in H1.
-    assert (k <= val v u); [clear H1|lia].
-    apply val_le_caract. destruct H2 as [e [H2 H2']].
-    exists e. split; tas. lia.
-Qed.
-
-Lemma val_add v e (s: Universe.t)
-  : val v (add e s) = Nat.max (val v e) (val v s).
-Proof.
-  apply val_caract. split.
-  - intros e' H. apply LevelExprSet.add_spec in H. destruct H as [H|H].
-    + subst. u; lia.
-    + eapply val_In_le with (v:=v) in H. lia.
-  - destruct (Nat.max_dec (val v e) (val v s)) as [H|H]; rewrite H; clear H.
-    + exists e. split; cbnr. apply LevelExprSetFact.add_1. reflexivity.
-    + destruct (val_In_max s v) as [e' [H1 H2]].
-      exists e'. split; tas. now apply LevelExprSetFact.add_2.
-Qed.
-
-Lemma val_sup v s1 s2 :
-  val v (Universe.sup s1 s2) = Nat.max (val v s1) (val v s2).
-Proof.
-  eapply val_caract. cbn. split.
-  - intros e' H. eapply LevelExprSet.union_spec in H. destruct H as [H|H].
-    + eapply val_In_le with (v:=v) in H. lia.
-    + eapply val_In_le with (v:=v) in H. lia.
-  - destruct (Nat.max_dec (val v s1) (val v s2)) as [H|H]; rewrite H; clear H.
-    + destruct (val_In_max s1 v) as [e' [H1 H2]].
-      exists e'. split; tas. apply LevelExprSet.union_spec. now left.
-    + destruct (val_In_max s2 v) as [e' [H1 H2]].
-      exists e'. split; tas. apply LevelExprSet.union_spec. now right.
-Qed.
-
-Ltac proper := let H := fresh in try (intros ? ? H; destruct H; reflexivity).
-
-Lemma for_all_elements (P : LevelExpr.t -> bool) u :
-  LevelExprSet.for_all P u = forallb P (LevelExprSet.elements u).
-Proof.
-  apply LevelExprSetFact.for_all_b; proper.
-Qed.
-
-
-Lemma universe_get_is_level_correct u l :
-  Universe.get_is_level u = Some l -> u = Universe.make' l.
-Proof.
-  intro H.
-  unfold Universe.get_is_level in *.
-  destruct (LevelExprSet.elements u) as [|l0 L] eqn:Hu1; [discriminate |].
-  destruct l0, L; try discriminate.
-  * destruct n; inversion H; subst.
-    apply eq_univ''; apply Hu1.
-  * destruct n; discriminate.
-Qed.
-
-
-Lemma sup0_comm x1 x2 :
-  Universe.sup x1 x2 = Universe.sup x2 x1.
-Proof.
-  apply eq_univ'; simpl. unfold LevelExprSet.Equal.
-  intros H. rewrite !LevelExprSet.union_spec. intuition.
-Qed.
-
-(*
-Lemma val_zero_exprs v (l : Universe.t) : 0 <= val v l.
-Proof.
-  rewrite val_fold_right.
-  destruct (Universe.exprs l) as [e u']; clear l; cbn.
-  induction (List.rev u'); simpl.
-  - destruct e as [npl_expr].
-    destruct npl_expr as [t b].
-    cbn.
-    assert (0 <= val v t) by apply Level.val_zero.
-    destruct b;lia.
-  - pose proof (LevelExpr.val_zero a v); lia.
-Qed. *)
-
-
-Module ConstraintType.
-  Inductive t_ : Set := Le (z : Z) | Eq.
-  Derive NoConfusion EqDec for t_.
-
-  Definition t := t_.
-  Definition eq : t -> t -> Prop := eq.
-  Definition eq_equiv : Equivalence eq := _.
-
-  Definition Le0 := Le 0.
-  Definition Lt := Le 1.
-
-  Inductive lt_ : t -> t -> Prop :=
-  | LeLe n m : (n < m)%Z -> lt_ (Le n) (Le m)
-  | LeEq n : lt_ (Le n) Eq.
-  Derive Signature for lt_.
-  Definition lt := lt_.
-
-  Global Instance lt_strorder : StrictOrder lt.
-  Proof.
-    constructor.
-    - intros []; intro X; inversion X. lia.
-    - intros ? ? ? X Y; invs X; invs Y; constructor. lia.
-  Qed.
-
-  Global Instance lt_compat : Proper (eq ==> eq ==> iff) lt.
-  Proof.
-    intros ? ? X ? ? Y; invs X; invs Y. reflexivity.
-  Qed.
-
-  Definition compare (x y : t) : comparison :=
-    match x, y with
-    | Le n, Le m => Z.compare n m
-    | Le _, Eq => Datatypes.Lt
-    | Eq, Eq => Datatypes.Eq
-    | Eq, _  => Datatypes.Gt
-    end.
-
-  Lemma compare_spec x y : CompareSpec (eq x y) (lt x y) (lt y x) (compare x y).
-  Proof.
-    destruct x, y; repeat constructor. simpl.
-    destruct (Z.compare_spec z z0); simpl; constructor.
-    subst; constructor. now constructor. now constructor.
-  Qed.
-
-  Lemma eq_dec x y : {eq x y} + {~ eq x y}.
-  Proof.
-    unfold eq. decide equality. apply Z.eq_dec.
-  Qed.
-End ConstraintType.
-
-Module UnivConstraint.
-  Definition t : Set := Level.t * ConstraintType.t * Level.t.
-
-  Definition eq : t -> t -> Prop := eq.
-  Definition eq_equiv : Equivalence eq := _.
-
-  Definition make l1 ct l2 : t := (l1, ct, l2).
-
-  Inductive lt_ : t -> t -> Prop :=
-  | lt_Level2 l1 t l2 l2' : Level.lt l2 l2' -> lt_ (l1, t, l2) (l1, t, l2')
-  | lt_Cstr l1 t t' l2 l2' : ConstraintType.lt t t' -> lt_ (l1, t, l2) (l1, t', l2')
-  | lt_Level1 l1 l1' t t' l2 l2' : Level.lt l1 l1' -> lt_ (l1, t, l2) (l1', t', l2').
-  Definition lt := lt_.
-
-  Lemma lt_strorder : StrictOrder lt.
-  Proof.
-    constructor.
-    - intros []; intro X; inversion X; subst;
-        try (eapply Level.lt_strorder; eassumption).
-      eapply ConstraintType.lt_strorder; eassumption.
-    - intros ? ? ? X Y; invs X; invs Y; constructor; tea.
-      etransitivity; eassumption.
-      2: etransitivity; eassumption.
-      eapply ConstraintType.lt_strorder; eassumption.
-  Qed.
-
-  Lemma lt_compat : Proper (eq ==> eq ==> iff) lt.
-  Proof.
-    intros ? ? X ? ? Y; invs X; invs Y. reflexivity.
-  Qed.
-
-  Definition compare : t -> t -> comparison :=
-    fun '(l1, t, l2) '(l1', t', l2') =>
-      compare_cont (Level.compare l1 l1')
-        (compare_cont (ConstraintType.compare t t')
-                    (Level.compare l2 l2')).
-
-  Lemma compare_spec x y
-    : CompareSpec (eq x y) (lt x y) (lt y x) (compare x y).
-  Proof.
-    destruct x as [[l1 t] l2], y as [[l1' t'] l2']; cbn.
-    destruct (Level.compare_spec l1 l1'); cbn; repeat constructor; tas.
-    invs H.
-    destruct (ConstraintType.compare_spec t t'); cbn; repeat constructor; tas.
-    invs H.
-    destruct (Level.compare_spec l2 l2'); cbn; repeat constructor; tas.
-    invs H. reflexivity.
-  Qed.
-
-  Lemma eq_dec x y : {eq x y} + {~ eq x y}.
-  Proof.
-    unfold eq. decide equality; apply eq_dec.
-  Defined.
-
-  Definition eq_leibniz (x y : t) : eq x y -> x = y := id.
-End UnivConstraint.
-
-Module ConstraintSet := MSetAVL.Make UnivConstraint.
-Module ConstraintSetFact := WFactsOn UnivConstraint ConstraintSet.
-Module ConstraintSetOrdProp := MSetProperties.OrdProperties ConstraintSet.
-Module ConstraintSetProp := ConstraintSetOrdProp.P.
-Module CS := ConstraintSet.
-Module ConstraintSetDecide := ConstraintSetProp.Dec.
-Module ConstraintSetExtraOrdProp := MSets.ExtraOrdProperties ConstraintSet ConstraintSetOrdProp.
-Module ConstraintSetExtraDecide := MSetAVL.Decide UnivConstraint ConstraintSet.
-Ltac csets := ConstraintSetDecide.fsetdec.
-
-Notation "(=_cset)" := ConstraintSet.Equal (at level 0).
-Infix "=_cset" := ConstraintSet.Equal (at level 30).
-Notation "(==_cset)" := ConstraintSet.equal (at level 0).
-Infix "==_cset" := ConstraintSet.equal (at level 30).
-
-Definition declared_cstr_levels levels (cstr : UnivConstraint.t) :=
-  let '(l1,_,l2) := cstr in
-  LevelSet.In l1 levels /\ LevelSet.In l2 levels.
-
-Definition is_declared_cstr_levels levels (cstr : UnivConstraint.t) : bool :=
-  let '(l1,_,l2) := cstr in
-  LevelSet.mem l1 levels && LevelSet.mem l2 levels.
-
-Lemma CS_union_empty s : ConstraintSet.union ConstraintSet.empty s =_cset s.
-Proof.
-  intros x; rewrite ConstraintSet.union_spec. lsets.
-Qed.
-
-Lemma CS_For_all_union f cst cst' : ConstraintSet.For_all f (ConstraintSet.union cst cst') ->
-  ConstraintSet.For_all f cst.
-Proof.
-  unfold CS.For_all.
-  intros IH x inx. apply (IH x).
-  now eapply CS.union_spec; left.
-Qed.
-
-Lemma CS_For_all_add P x s : CS.For_all P (CS.add x s) -> P x /\ CS.For_all P s.
-Proof.
-  intros.
-  split.
-  * apply (H x), CS.add_spec; left => //.
-  * intros y iny. apply (H y), CS.add_spec; right => //.
-Qed.
-
-#[global] Instance CS_For_all_proper P : Morphisms.Proper ((=_cset) ==> iff)%signature (ConstraintSet.For_all P).
-Proof.
-  intros s s' eqs.
-  unfold CS.For_all. split; intros IH x inxs; apply (IH x);
-  now apply eqs.
-Qed.
-
-(** {6 Sort instances} *)
-
-Module Instance.
-
-  (** A universe instance represents a vector of argument concrete_sort
-      to a polymorphic definition (constant, inductive or constructor). *)
-  Definition t : Set := list Level.t.
-
-  Definition empty : t := [].
-  Definition is_empty (i : t) : bool :=
-    match i with
-    | [] => true
-    | _ => false
-    end.
-
-  Definition eqb (i j : t) :=
-    forallb2 Level.eqb i j.
-
-  Definition equal_upto (f : Level.t -> Level.t -> bool) (i j : t) :=
-    forallb2 f i j.
-End Instance.
-
-Module UContext.
-  Definition t := list name × (Instance.t × ConstraintSet.t).
-
-  Definition make' : Instance.t -> ConstraintSet.t -> Instance.t × ConstraintSet.t := pair.
-  Definition make (ids : list name) (inst_ctrs : Instance.t × ConstraintSet.t) : t := (ids, inst_ctrs).
-
-  Definition empty : t := ([], (Instance.empty, ConstraintSet.empty)).
-
-  Definition instance : t -> Instance.t := fun x => fst (snd x).
-  Definition constraints : t -> ConstraintSet.t := fun x => snd (snd x).
-
-  Definition dest : t -> list name * (Instance.t * ConstraintSet.t) := fun x => x.
-End UContext.
-
-Module AUContext.
-  Definition t := list name × ConstraintSet.t.
-
-  Definition make (ids : list name) (ctrs : ConstraintSet.t) : t := (ids, ctrs).
-  Definition repr (x : t) : UContext.t :=
-    let (u, cst) := x in
-    (u, (mapi (fun i _ => Level.lvar i) u, cst)).
-
-  Definition levels (uctx : t) : LevelSet.t :=
-    LevelSetProp.of_list (fst (snd (repr uctx))).
-
-  #[local]
-  Existing Instance EqDec_ReflectEq.
-  Definition inter (au av : AUContext.t) : AUContext.t :=
-    let prefix := (split_prefix au.1 av.1).1.1 in
-    let lvls := fold_left_i (fun s i _ => LevelSet.add (Level.lvar i) s) prefix LevelSet.empty in
-    let filter := ConstraintSet.filter (is_declared_cstr_levels lvls) in
-    make prefix (ConstraintSet.union (filter au.2) (filter av.2)).
-End AUContext.
-
-Module ContextSet.
-  Definition t := LevelSet.t × ConstraintSet.t.
-
-  Definition levels : t -> LevelSet.t := fst.
-  Definition constraints : t -> ConstraintSet.t := snd.
-
-  Definition empty : t := (LevelSet.empty, ConstraintSet.empty).
-
-  Definition is_empty (uctx : t)
-    := LevelSet.is_empty (fst uctx) && ConstraintSet.is_empty (snd uctx).
-
-  Definition Equal (x y : t) : Prop :=
-    x.1 =_lset y.1 /\ x.2 =_cset y.2.
-
-  Definition equal (x y : t) : bool :=
-    x.1 ==_lset y.1 && x.2 ==_cset y.2.
-
-  Definition Subset (x y : t) : Prop :=
-    LevelSet.Subset (levels x) (levels y) /\
-    ConstraintSet.Subset (constraints x) (constraints y).
-
-  Definition subset (x y : t) : bool :=
-    LevelSet.subset (levels x) (levels y) &&
-    ConstraintSet.subset (constraints x) (constraints y).
-
-  Definition inter (x y : t) : t :=
-    (LevelSet.inter (levels x) (levels y),
-      ConstraintSet.inter (constraints x) (constraints y)).
-
-  Definition inter_spec (x y : t) :
-    Subset (inter x y) x /\
-      Subset (inter x y) y /\
-      forall z, Subset z x -> Subset z y -> Subset z (inter x y).
-  Proof.
-    split; last split.
-    1,2: split=> ?; [move=> /LevelSet.inter_spec [//]|move=> /ConstraintSet.inter_spec [//]].
-    move=> ? [??] [??]; split=> ??;
-    [apply/LevelSet.inter_spec|apply/ConstraintSet.inter_spec]; split; auto.
-  Qed.
-
-  Definition union (x y : t) : t :=
-    (LevelSet.union (levels x) (levels y), ConstraintSet.union (constraints x) (constraints y)).
-
-  Definition union_spec (x y : t) :
-    Subset x (union x y) /\
-      Subset y (union x y) /\
-      forall z, Subset x z -> Subset y z -> Subset (union x y) z.
-  Proof.
-    split; last split.
-    1,2: split=> ??; [apply/LevelSet.union_spec|apply/ConstraintSet.union_spec ]; by constructor.
-    move=> ? [??] [??]; split=> ?;
-    [move=>/LevelSet.union_spec|move=>/ConstraintSet.union_spec]=>-[]; auto.
-  Qed.
-
-  Lemma equal_spec s s' : equal s s' <-> Equal s s'.
-  Proof.
-    rewrite /equal/Equal/is_true Bool.andb_true_iff LevelSet.equal_spec ConstraintSet.equal_spec.
-    reflexivity.
-  Qed.
-
-  Lemma subset_spec s s' : subset s s' <-> Subset s s'.
-  Proof.
-    rewrite /subset/Subset/is_true Bool.andb_true_iff LevelSet.subset_spec ConstraintSet.subset_spec.
-    reflexivity.
-  Qed.
-
-  Lemma subsetP s s' : reflect (Subset s s') (subset s s').
-  Proof.
-    generalize (subset_spec s s').
-    destruct subset; case; constructor; intuition.
-  Qed.
-End ContextSet.
-
-Export (hints) ContextSet.
-
-Notation "(=_cs)" := ContextSet.Equal (at level 0).
-Notation "(⊂_cs)" := ContextSet.Subset (at level 0).
-Infix "=_cs" := ContextSet.Equal (at level 30).
-Infix "⊂_cs" := ContextSet.Subset (at level 30).
-Notation "(==_cs)" := ContextSet.equal (at level 0).
-Notation "(⊂?_cs)" := ContextSet.subset (at level 0).
-Infix "==_cs" := ContextSet.equal (at level 30).
-Infix "⊂?_cs" := ContextSet.subset (at level 30).
-
-Lemma incl_cs_refl cs : cs ⊂_cs cs.
-Proof.
-  split; [lsets|csets].
-Qed.
-
-Lemma incl_cs_trans cs1 cs2 cs3 : cs1 ⊂_cs cs2 -> cs2 ⊂_cs cs3 -> cs1 ⊂_cs cs3.
-Proof.
-  intros [? ?] [? ?]; split; [lsets|csets].
-Qed.
-
-Lemma empty_contextset_subset u : ContextSet.empty ⊂_cs u.
-Proof.
-  red. split; cbn; [lsets|csets].
-Qed.
-
-(* Variance info is needed to do full universe polymorphism *)
-Module Variance.
-  (** A universe position in the instance given to a cumulative
-     inductive can be the following. Note there is no Contralvariant
-     case because [forall x : A, B <= forall x : A', B'] requires [A =
-     A'] as opposed to [A' <= A]. *)
-  Inductive t :=
-  | Irrelevant : t
-  | Covariant : t
-  | Invariant : t.
-  Derive NoConfusion EqDec for t.
-
-  (* val check_subtype : t -> t -> bool *)
-  (* val sup : t -> t -> t *)
-End Variance.
-
-(** What to check of two instances *)
-Variant opt_variance :=
-  AllEqual | AllIrrelevant | Variance of list Variance.t.
-
-Inductive universes_decl : Type :=
-| Monomorphic_ctx
-| Polymorphic_ctx (cst : AUContext.t).
-
-Derive NoConfusion for universes_decl.
-
-Definition levels_of_udecl u :=
-  match u with
-  | Monomorphic_ctx => LevelSet.empty
-  | Polymorphic_ctx ctx => AUContext.levels ctx
-  end.
-
-Definition constraints_of_udecl u :=
-  match u with
-  | Monomorphic_ctx => ConstraintSet.empty
-  | Polymorphic_ctx ctx => snd (snd (AUContext.repr ctx))
-  end.
-
-Declare Scope univ_scope.
-Delimit Scope univ_scope with u.
-
-Inductive satisfies0 (v : valuation) : UnivConstraint.t -> Prop :=
-| satisfies0_Lt (l l' : Level.t) (z : Z) : (Z.of_nat (val v l) <= Z.of_nat (val v l') - z)%Z
-                        -> satisfies0 v (l, ConstraintType.Le z, l')
-| satisfies0_Eq (l l' : Level.t) : val v l = val v l'
-                        -> satisfies0 v (l, ConstraintType.Eq, l').
-
-Definition satisfies v : ConstraintSet.t -> Prop :=
-  ConstraintSet.For_all (satisfies0 v).
-
-Lemma satisfies_union v φ1 φ2 :
-  satisfies v (CS.union φ1 φ2)
-  <-> (satisfies v φ1 /\ satisfies v φ2).
-Proof using Type.
-  unfold satisfies. split.
-  - intros H; split; intros c Hc; apply H; now apply CS.union_spec.
-  - intros [H1 H2] c Hc; apply CS.union_spec in Hc; destruct Hc; auto.
-Qed.
-
-Lemma satisfies_subset φ φ' val :
-  ConstraintSet.Subset φ φ' ->
-  satisfies val φ' ->
-  satisfies val φ.
-Proof using Type.
-  intros sub sat ? isin.
-  apply sat, sub; auto.
-Qed.
-
-Definition consistent ctrs := exists v, satisfies v ctrs.
-
-Definition consistent_extension_on cs cstr :=
-  forall v, satisfies v (ContextSet.constraints cs) -> exists v',
-      satisfies v' cstr /\
-        LevelSet.For_all (fun l => val v l = val v' l) (ContextSet.levels cs).
-
-Lemma consistent_extension_on_empty Σ :
-  consistent_extension_on Σ CS.empty.
-Proof using Type.
-  move=> v hv; exists v; split; [move=> ? /CS.empty_spec[]| move=> ??//].
-Qed.
-
-Lemma consistent_extension_on_union X cstrs
-  (wfX : forall c, CS.In c X.2 -> LS.In c.1.1 X.1 /\ LS.In c.2 X.1) :
-  consistent_extension_on X cstrs <->
-  consistent_extension_on X (CS.union cstrs X.2).
-Proof using Type.
-  split.
-  2: move=> h v /h [v' [/satisfies_union [??] eqv']]; exists v'; split=> //.
-  move=> hext v /[dup] vsat /hext [v' [v'sat v'eq]].
-  exists v'; split=> //.
-  apply/satisfies_union; split=> //.
-  move=> c hc. destruct (wfX c hc).
-  destruct (vsat c hc); constructor; rewrite -!v'eq //.
-Qed.
-
-
-Definition leq0_universe_n n φ (u u' : Universe.t) :=
-  forall v, satisfies v φ -> (Z.of_nat (val v u) <= Z.of_nat (val v u') - n)%Z.
-
-Definition leq_universe_n {cf} n φ (u u' : Universe.t) :=
-  if check_univs then leq0_universe_n n φ u u' else True.
-
-Definition lt_universe {cf} := leq_universe_n 1.
-Definition leq_universe {cf} := leq_universe_n 0.
-
-Definition eq0_universe φ (u u' : Universe.t) :=
-  forall v, satisfies v φ -> val v u = val v u'.
-
-Definition eq_universe {cf} φ (u u' : Universe.t) :=
-  if check_univs then eq0_universe φ u u' else True.
-
-(* ctrs are "enforced" by φ *)
-
-Definition valid_constraints0 φ ctrs
-  := forall v, satisfies v φ -> satisfies v ctrs.
-
-Definition valid_constraints {cf} φ ctrs
-  := if check_univs then valid_constraints0 φ ctrs else True.
-
-Definition compare_universe {cf} φ (pb : conv_pb) :=
-  match pb with
-  | Conv => eq_universe φ
-  | Cumul => leq_universe φ
-  end.
-
-
-Ltac unfold_univ_rel0 :=
-  unfold eq0_universe, leq0_universe_n, valid_constraints0 in *;
-  try (
-    match goal with |- forall v : valuation, _ -> _ => idtac end;
-    intros v Hv;
-    repeat match goal with H : forall v : valuation, _ -> _ |- _ => specialize (H v Hv) end;
-    cbnr
-  ).
-
-Ltac unfold_univ_rel :=
-  unfold eq_universe, leq_universe, lt_universe, leq_universe_n, valid_constraints in *;
-  destruct check_univs; [unfold_univ_rel0 | trivial].
-
-Section Univ.
-  Context {cf}.
-
-  Lemma valid_subset φ φ' ctrs
-    : ConstraintSet.Subset φ φ' -> valid_constraints φ ctrs
-      ->  valid_constraints φ' ctrs.
-  Proof using Type.
-    unfold_univ_rel.
-    intros Hφ H v Hv. apply H.
-    intros ctr Hc. apply Hv. now apply Hφ.
-  Qed.
-
-  Lemma switch_minus (x y z : Z) : (x <= y - z <-> x + z <= y)%Z.
-  Proof using Type. split; lia. Qed.
-
-  (** **** Lemmas about eq and leq **** *)
-
-  Global Instance eq_universe_refl φ : Reflexive (eq_universe φ).
-  Proof using Type.
-    intros u; unfold_univ_rel.
-  Qed.
-
-  Global Instance leq_universe_refl φ : Reflexive (leq_universe φ).
-  Proof using Type.
-    intros u; unfold_univ_rel. lia.
-  Qed.
-
-  Global Instance eq_universe_sym φ : Symmetric (eq_universe φ).
-  Proof using Type.
-    intros u u' H; unfold_univ_rel.
-    lia.
-  Qed.
-
-  Global Instance eq_universe_trans φ : Transitive (eq_universe φ).
-  Proof using Type.
-    intros u u' u'' H1 H2; unfold_univ_rel.
-    lia.
-  Qed.
-
-  Global Instance leq_universe_n_trans n φ : Transitive (leq_universe_n (Z.of_nat n) φ).
-  Proof using Type.
-    intros u u' u'' H1 H2; unfold_univ_rel.
-    lia.
-  Qed.
-
-  Global Instance leq_universe_trans φ : Transitive (leq_universe φ).
-  Proof using Type. apply (leq_universe_n_trans 0). Qed.
-
-  Global Instance lt_universe_trans φ : Transitive (lt_universe φ).
-  Proof using Type. apply (leq_universe_n_trans 1). Qed.
-
-  Lemma eq0_leq0_universe φ u u' :
-    eq0_universe φ u u' <-> leq0_universe_n 0 φ u u' /\ leq0_universe_n 0 φ u' u.
-  Proof using Type.
-    split.
-    - intros H. split; unfold_univ_rel0; lia.
-    - intros [H1 H2]. unfold_univ_rel0; lia.
-  Qed.
-
-  Lemma eq_universe_leq_universe φ u u' :
-    eq_universe φ u u' <-> leq_universe φ u u' /\ leq_universe φ u' u.
-  Proof using Type.
-    unfold_univ_rel => //.
-    apply eq0_leq0_universe.
-  Qed.
-
-  Lemma leq_universe_sup_l φ u1 u2 : leq_universe φ u1 (Universe.sup u1 u2).
-  Proof using Type. unfold_univ_rel. rewrite val_sup; lia. Qed.
-
-  Lemma leq_universe_sup_r φ u1 u2 : leq_universe φ u2 (Universe.sup u1 u2).
-  Proof using Type. unfold_univ_rel. rewrite val_sup; lia. Qed.
-
-  Lemma leq_universe_sup_mon φ u1 u1' u2 u2' : leq_universe φ u1 u1' -> leq_universe φ u2 u2' ->
-    leq_universe φ (Universe.sup u1 u2) (Universe.sup u1' u2').
-  Proof using Type.
-    intros H1 H2; unfold_univ_rel.
-    rewrite !val_sup. lia.
-  Qed.
-
-  Global Instance eq_leq_universe φ : subrelation (eq_universe φ) (leq_universe φ).
-  Proof using Type.
-    intros u u'. apply eq_universe_leq_universe.
-  Qed.
-
-  Global Instance eq_universe_equivalence φ : Equivalence (eq_universe φ) := Build_Equivalence _ _ _ _.
-
-  Global Instance leq_universe_preorder φ : PreOrder (leq_universe φ) := Build_PreOrder _ _ _.
-
-  Global Instance lt_universe_irrefl {c: check_univs} φ (H: consistent φ) : Irreflexive (lt_universe φ).
-  Proof using Type.
-    intro u. unfold complement.
-    unfold_univ_rel => //.
-    destruct H as [v Hv]; intros nH; specialize (nH v Hv); lia.
-  Qed.
-
-  Global Instance lt_universe_str_order {c: check_univs} φ (H: consistent φ) : StrictOrder (lt_universe φ).
-  Proof.
-    refine (Build_StrictOrder _ _ _).
-    now unshelve eapply lt_universe_irrefl.
-  Qed.
-
-  Global Instance leq_universe_antisym φ : Antisymmetric _ (eq_universe φ) (leq_universe φ).
-  Proof using Type. intros t u tu ut. now apply eq_universe_leq_universe. Qed.
-
-  Global Instance leq_universe_partial_order φ
-    : PartialOrder (eq_universe φ) (leq_universe φ).
-  Proof.
-    intros x y; split; apply eq_universe_leq_universe.
-  Defined.
-
-
-  Global Instance compare_universe_subrel φ pb : subrelation (eq_universe φ) (compare_universe φ pb).
-  Proof using Type.
-    destruct pb; tc.
-  Qed.
-
-  Global Instance compare_universe_refl φ pb : Reflexive (compare_universe φ pb).
-  Proof using Type.
-    destruct pb; tc.
-  Qed.
-
-  Global Instance compare_universe_trans φ pb : Transitive (compare_universe φ pb).
-  Proof using Type.
-    destruct pb; tc.
-  Qed.
-
-  Global Instance compare_universe_preorder φ pb : PreOrder (compare_universe φ pb).
-  Proof using Type.
-    destruct pb; tc.
-  Qed.
-
-  Definition eq_leq_universe' φ u u'
-    := @eq_leq_universe φ u u'.
-  Definition leq_universe_refl' φ u
-    := @leq_universe_refl φ u.
-
-  Hint Resolve eq_leq_universe' leq_universe_refl' : core.
-
-
-  Lemma cmp_universe_subset φ φ' pb t u :
-    ConstraintSet.Subset φ φ' -> compare_universe φ pb t u -> compare_universe φ' pb t u.
-  Proof using Type.
-    intros Hctrs.
-    destruct pb, t, u; cbnr; trivial.
-    all: intros H; unfold_univ_rel;
-    apply H.
-    all: eapply satisfies_subset; eauto.
-  Qed.
-
-  Lemma eq_universe_subset φ φ' t u
-    : ConstraintSet.Subset φ φ'
-      -> eq_universe φ t u -> eq_universe φ' t u.
-  Proof using Type. apply cmp_universe_subset with (pb := Conv). Qed.
-
-  Lemma leq_universe_subset φ φ' t u
-    : ConstraintSet.Subset φ φ'
-      -> leq_universe φ t u -> leq_universe φ' t u.
-  Proof using Type. apply cmp_universe_subset with (pb := Cumul). Qed.
-
-End Univ.
-
-Module Sort.
-  Inductive t_ {univ} :=
-    sProp | sSProp | sType (_ : univ).
-  Derive NoConfusion for t_.
-  Arguments t_ : clear implicits.
-
-  Definition t := t_ Universe.t.
-
-  Inductive family : Set :=
-  | fSProp
-  | fProp
-  | fType.
-  Derive NoConfusion EqDec for family.
-
-  Definition eqb {univ} `{ReflectEq univ} (u1 u2 : t_ univ) : bool :=
-    match u1, u2 with
-    | sSProp, sSProp => true
-    | sProp, sProp => true
-    | sType e1, sType e2 => eqb e1 e2
-    | _, _ => false
-    end.
-
-  #[global, program] Instance reflect_eq_sort {univ} `{ReflectEq univ} : ReflectEq (t_ univ) :=
-    { eqb := eqb }.
-  Next Obligation.
-    destruct x, y; cbn; try constructor; auto; try congruence.
-    destruct (eqb_spec u u0); constructor. now f_equal.
-    congruence.
-  Qed.
-
-  #[global] Instance eq_dec_sort {univ} `{EqDec univ} : EqDec (t_ univ) := ltac:(intros s s'; decide equality).
-
-  Definition map {u u'} (f : u -> u') s :=
-    match s with
-    | sType u => sType (f u)
-    | sProp => sProp
-    | sSProp => sSProp
-    end.
-
-  Definition on_sort {univ} {T} (P: univ -> T) (def: T) (s : t_ univ) :=
-    match s with
-    | sProp | sSProp => def
-    | sType l => P l
-    end.
-
-  (** Test if the universe is a lub of levels or contains +n's. *)
-  Definition is_levels (s : t) : bool :=
-    match s with
+    match u.(s) with
     | sSProp | sProp => true
-    | sType l => Universe.is_levels l
+    | sType => UnivLvl.is_level u.(l)
     end.
 
-  (** Test if the universe is a level or an algebraic universe. *)
-  Definition is_level (s : t) : bool :=
-    match s with
-    | sSProp | sProp => true
-    | sType l => Universe.is_level l
-    end.
-
-  Definition is_sprop {univ} (s : t_ univ) : bool :=
-    match s with
+  Definition is_sprop {ulvl} (u : t_ Sort.t ulvl) : bool :=
+    match u.(s) with
       | sSProp => true
       | _ => false
     end.
 
-  Definition is_prop {univ} (s : t_ univ) : bool :=
-    match s with
+  Definition is_prop {ulvl} (u : t_ Sort.t ulvl) : bool :=
+    match u.(s) with
       | sProp => true
       | _ => false
     end.
 
-  Definition is_propositional {univ} (s : t_ univ) : bool :=
-    match s with
+  Definition is_propositional {ulvl} (u : t_ Sort.t ulvl) : bool :=
+    match u.(s) with
       | sProp | sSProp => true
       | _ => false
     end.
 
-  Lemma is_prop_propositional {univ} (s : t_ univ) :
-    is_prop s -> is_propositional s.
-  Proof. now destruct s. Qed.
-  Lemma is_sprop_propositional {univ} (s : t_ univ) :
-    is_sprop s -> is_propositional s.
-  Proof. now destruct s. Qed.
+  Lemma is_prop_propositional {ulvl} (u : t_ Sort.t ulvl) :
+    is_prop u -> is_propositional u.
+  Proof. destruct u as [s l]; now destruct s. Qed.
+  Lemma is_sprop_propositional {ulvl} (u : t_ Sort.t ulvl) :
+    is_sprop u -> is_propositional u.
+  Proof. destruct u as [s l]; now destruct s. Qed.
 
-  Definition is_type_sort {univ} (s : t_ univ) : bool :=
-    match s with
-      | sType _ => true
+  Definition is_type_sort {ulvl} (u : t_ Sort.t ulvl) : bool :=
+    match u.(s) with
+      | sType => true
       | _ => false
     end.
 
-  Definition type0 : t := sType (Universe.make LevelExpr.set).
-  Definition type1 : t := sType (Universe.make LevelExpr.type1).
+  Definition type0 : t := mk sType UnivLvl.type0.
+  Definition type1 : t := mk sType UnivLvl.type1.
 
   Definition of_levels (l : PropLevel.t + Level.t) : t :=
     match l with
-    | inl PropLevel.lSProp => sSProp
-    | inl PropLevel.lProp => sProp
-    | inr l => sType (Universe.make' l)
+    | inl PropLevel.lSProp => mk sSProp UnivLvl.type0
+    | inl PropLevel.lProp => mk sProp UnivLvl.type0
+    | inr l => mk sType (UnivLvl.make' l)
     end.
 
   (** The universe strictly above FOR TYPING (not cumulativity) *)
 
-  Definition super_ {univ} type1 univ_succ (s : t_ univ) : t_ univ :=
-    match s with
-    | sSProp | sProp => sType type1
-    | sType l => sType (univ_succ l)
+  Definition super_ {ulvl} type1 usucc (u : t_ Sort.t ulvl) : t_ Sort.t ulvl :=
+    match u.(s) with
+    | sSProp | sProp => mk sType type1
+    | sType => mk sType (usucc u.(l))
     end.
-  Definition super : t -> t := super_ (Universe.make LevelExpr.type1) Universe.succ.
+  Definition super : t -> t := super_ UnivLvl.type1 UnivLvl.succ.
   Definition csuper := super_ 1 S.
 
-  Definition sup_ {univ} univ_sup (s s' : t_ univ) : t_ univ :=
-    match s, s' with
-    | sSProp, s' => s'
-    | sProp, sSProp => sProp
-    | sProp, s' => s'
-    | sType u1, sType u2 => sType (univ_sup u1 u2)
-    | sType _ as s, _ => s
+  Definition sup_ {ulvl} type0 univ_sup (u u' : t_ Sort.t ulvl) : t_ Sort.t ulvl :=
+    match u.(s), u'.(s) with
+    | sSProp, sSProp => mk sSProp type0
+    | sSProp, sProp | sProp, sSProp => mk sProp type0
+    | sSProp, _ => u'
+    | _, sSProp => u
+    | sProp, sProp => mk sProp type0
+    | sProp, _ => u'
+    | _, sProp => u
+    | sType, sType => mk sType (univ_sup u.(l) u'.(l))
     end.
-  Definition sup : t -> t -> t := sup_ Universe.sup.
-  Definition csup := sup_ Nat.max.
+  Definition sup : t -> t -> t := sup_ UnivLvl.type0 UnivLvl.sup.
+  Definition csup := sup_ 0 Nat.max.
 
   (** Type of a product *)
-  Definition sort_of_product_ {univ} univ_sup (domsort rangsort : t_ univ) : t_ univ :=
-    match rangsort with
-    | sSProp | sProp => rangsort
+  Definition univ_of_product_ {ulvl} type0 usup (dom codom : t_ Sort.t ulvl) : t_ Sort.t ulvl :=
+    match codom.(s) with
+    | sSProp | sProp => codom
     (* Prop and SProp impredicativity *)
-    | _ => Sort.sup_ univ_sup domsort rangsort
+    | _ => sup_ type0 usup dom codom
     end.
-  Definition sort_of_product : t -> t -> t := sort_of_product_ Universe.sup.
-  Definition csort_of_product := sort_of_product_ Nat.max.
+  Definition univ_of_product : t -> t -> t := univ_of_product_ UnivLvl.type0 UnivLvl.sup.
+  Definition cuniv_of_product := univ_of_product_ 0 Nat.max.
 
-  Definition get_is_level (s : t) : option Level.t :=
-    match s with
+  Definition get_is_level (u : t) : option Level.t :=
+    match u.(s) with
     | sSProp => None
     | sProp => None
-    | sType l => Universe.get_is_level l
+    | sType => UnivLvl.get_is_level u.(l)
     end.
 
-  Definition to_family {univ} (s : t_ univ) :=
-    match s with
-    | sSProp => fSProp
-    | sProp => fProp
-    | sType _ => fType
-    end.
+  Definition to_family {sort ulvl} (u : t_ sort ulvl) := u.(s).
 
-  Definition to_csort v s :=
-    match s with
-    | sSProp => sSProp
-    | sProp => sProp
-    | sType u => sType (val v u)
-    end.
+  Definition to_csort v (u : t) := mk u.(s) (val v u.(l)).
 
-  Lemma to_family_to_csort s v :
-    to_family (to_csort v s) = to_family s.
+  Lemma to_family_to_csort u v :
+    to_family (to_csort v u) = to_family u.
   Proof.
-    destruct s; cbnr.
+    destruct u as [s l]; unfold to_csort; destruct s; cbnr.
   Qed.
 
-  Lemma sType_super_ {univ type1 univ_succ} (s : t_ univ) :
-    to_family (super_ type1 univ_succ s) = fType.
-  Proof. now destruct s. Qed.
+  Lemma sType_super_ {ulvl type1 usucc} (u : t_ Sort.t ulvl) :
+    to_family (super_ type1 usucc u) = sType.
+  Proof. destruct u as [s l]; now destruct s. Qed.
 
   Lemma sType_super (s : t) :
-    to_family (super s) = fType.
+    to_family (super s) = sType.
   Proof. apply sType_super_. Qed.
 
-  Inductive lt_ {univ univ_lt} : t_ univ -> t_ univ -> Prop :=
-  | ltPropSProp : lt_ sProp sSProp
-  | ltPropType s : lt_ sProp (sType s)
-  | ltSPropType s : lt_ sSProp (sType s)
-  | ltTypeType s1 s2 : univ_lt s1 s2 -> lt_ (sType s1) (sType s2).
-  Derive Signature for lt_.
-  Arguments lt_ {univ} univ_lt.
+  Definition lt_ {sort ulvl} slt eqs ult (u v : t_ sort ulvl) : Prop :=
+    slt u.(s) v.(s) \/
+	(eqs u.(s) v.(s) /\ ult u.(l) v.(l)).
 
-  Definition lt := lt_ Universe.lt.
-  Definition clt := lt_ Nat.lt.
+  Definition lt := lt_ Sort.lt eq UnivLvl.lt.
+  Definition clt := lt_ Sort.lt eq Nat.lt.
 
   Module OT <: OrderedType.
     Definition t := t.
@@ -1639,334 +192,316 @@ Module Sort.
     #[local] Instance lt_strorder : StrictOrder lt.
     Proof.
       constructor.
-      - intros [| |] X; inversion X.
-        now eapply irreflexivity in H1.
-      - intros [| |] [| |] [| |] X1 X2;
-          inversion X1; inversion X2; constructor.
-        subst.
-        etransitivity; tea.
+      - intros [s l] [contra | [_ contra]]; cbn in *;
+	    by apply irreflexivity in contra.
+	  - intros [s1 l1] [s2 l2] [s3 l3] [hslt | [he hlt]] [hslt' | [he' hlt']]; cbn in *.
+	    + left. etransitivity; eauto.
+		+ left. by rewrite -he'. 
+		+ left. by rewrite he.
+		+ right; split; cbn.
+		  * congruence.
+		  * etransitivity; eauto.
     Qed.
 
     Definition lt_compat : Proper (eq ==> eq ==> iff) lt.
     Proof.
       intros x y e z t e'. hnf in * |- ; subst. reflexivity.
     Qed.
-    Definition compare (x y : t) : comparison
-      := match x, y with
-          | sProp, sProp => Eq
-          | sProp, _ => Lt
-          | _, sProp => Gt
-          | sSProp, sSProp => Eq
-          | sSProp, _ => Lt
-          | _, sSProp => Gt
-          | sType x, sType y => LevelExprSet.compare x y
-          end.
+	
+    Definition compare (u v : t) : comparison :=
+	  match Sort.compare u.(s) v.(s) with
+	  | Eq => LevelExprSet.compare u.(l) v.(l)
+	  | _ as c => c
+	  end.
+
     Lemma compare_spec x y : CompareSpec (eq x y) (lt x y) (lt y x) (compare x y).
     Proof.
-      cbv [compare eq].
-      destruct x, y.
-      all: lazymatch goal with
-            | [ |- context[LevelExprSet.compare ?x ?y] ]
-              => destruct (LevelExprSet.compare_spec x y)
-            | _ => idtac
-            end.
-      all: lazymatch goal with
-            | [ H : LevelExprSet.eq (?f ?x) (?f ?y) |- _ ]
-              => apply LevelExprSet.eq_leibniz in H;
-                is_var x; is_var y; destruct x, y; cbn in H; subst
-            | _ => idtac
-            end.
-      all: repeat constructor; try apply f_equal; try assumption.
-      f_equal; apply Eqdep_dec.UIP_dec; decide equality.
+	  destruct x as [s l], y as [s' l']; cbv [compare eq]; cbn.
+	  destruct (Sort.compare_spec s s').
+	  (* Only the case Eq needs more justification. *)
+	  2,3: constructor; cbv[lt Universe.lt lt_]; now left.
+	  subst; destruct (LevelExprSet.compare_spec l l'); cbn; constructor.
+	  - apply univ_eq; cbn; auto.
+	    apply NonEmptySetFacts.eq_univ', H.
+	  - cbv[lt Universe.lt lt_]; cbn.
+	    right; split; auto.
+	  - cbv[lt Universe.lt lt_]; cbn.
+	    right; split; auto.
     Qed.
+
     Definition eq_dec (x y : t) : {x = y} + {x <> y}.
-    Proof. repeat decide equality. apply Universe.eq_dec_univ0. Defined.
+    Proof. repeat decide equality. apply UnivLvl.eq_dec_univ0. Defined.
   End OT.
   Module OTOrig <: OrderedTypeOrig := Backport_OT OT.
-End Sort.
+End Universe.
 
 
-Module SortMap := FMapAVL.Make Sort.OTOrig.
-Module SortMapFact := FMapFacts.WProperties SortMap.
-Module SortMapExtraFact := FSets.WFactsExtra_fun Sort.OTOrig SortMap SortMapFact.F.
-Module SortMapDecide := FMapAVL.Decide Sort.OTOrig SortMap.
+Module UnivMap := FMapAVL.Make Universe.OTOrig.
+Module UnivMapFact := FMapFacts.WProperties UnivMap.
+Module UnivMapExtraFact := FSets.WFactsExtra_fun Universe.OTOrig UnivMap UnivMapFact.F.
+Module UnivMapDecide := FMapAVL.Decide Universe.OTOrig UnivMap.
 
-Notation sProp := Sort.sProp.
-Notation sSProp := Sort.sSProp.
-Notation sType := Sort.sType.
-Notation sort := Sort.t.
+Notation usort := Universe.s.
+Notation ulvl := Universe.l.
 
-Notation "⟦ u ⟧_ v" := (Sort.to_csort v u) (at level 0, format "⟦ u ⟧_ v", v name) : univ_scope.
+Notation "⟦ u ⟧_ v" := (Universe.to_csort v u) (at level 0, format "⟦ u ⟧_ v", v name) : univ_scope.
 
 
-Lemma val_sort_sup v s1 s2 :
-  Sort.to_csort v (Sort.sup s1 s2) = Sort.csup (Sort.to_csort v s1) (Sort.to_csort v s2).
+Lemma val_sort_sup v u1 u2 :
+  Universe.to_csort v (Universe.sup u1 u2) =
+  Universe.csup (Universe.to_csort v u1) (Universe.to_csort v u2).
 Proof.
-  destruct s1 as [ | | u1]; destruct s2 as [ | | u2]; cbnr.
-  f_equal. apply val_sup.
+  destruct u1 as [[| |] l1], u2 as [[| |] l2]; cbv[Universe.to_csort]; cbnr; f_equal.
+  all: apply val_sup.
 Qed.
 
-Lemma is_prop_val s :
-  Sort.is_prop s -> forall v, Sort.to_csort v s = Sort.sProp.
-Proof.
-  destruct s => //.
-Qed.
+Lemma is_prop_val u :
+  Universe.is_prop u -> forall v, Universe.to_csort v u = Universe.mk sProp (val v (ulvl u)).
+Proof. destruct u as [[| |] l] => //. Qed.
 
-Lemma is_sprop_val s :
-  Sort.is_sprop s -> forall v, Sort.to_csort v s = Sort.sSProp.
-Proof.
-  destruct s => //.
-Qed.
+Lemma is_sprop_val u :
+  Universe.is_sprop u -> forall v, Universe.to_csort v u = Universe.mk sSProp (val v (ulvl u)).
+Proof. destruct u as [[| |] l] => //. Qed.
 
+Lemma val_is_prop u v :
+  Universe.to_csort v u = Universe.mk sProp (val v (ulvl u)) <-> Universe.is_prop u.
+Proof. destruct u as [[| |] l] => //. Qed.
 
-Lemma val_is_prop s v :
-  Sort.to_csort v s = sProp <-> Sort.is_prop s.
-Proof.
-  destruct s => //.
-Qed.
+Lemma val_is_sprop u v :
+  Universe.to_csort v u = Universe.mk sSProp (val v (ulvl u)) <-> Universe.is_sprop u.
+Proof. destruct u as [[| |] l] => //. Qed.
 
-Lemma val_is_sprop s v :
-  Sort.to_csort v s = sSProp <-> Sort.is_sprop s.
-Proof.
-  destruct s => //.
-Qed.
-
-Lemma is_prop_and_is_sprop_val_false s :
-  Sort.is_prop s = false -> Sort.is_sprop s = false ->
-  forall v, ∑ n, Sort.to_csort v s = sType n.
+Lemma is_prop_and_is_sprop_val_false u :
+  Universe.is_prop u = false -> Universe.is_sprop u = false ->
+  forall v, ∑ n, Universe.to_csort v u = Universe.mk sType n.
 Proof.
   intros Hp Hsp v.
-  destruct s => //. simpl. eexists; eauto.
+  destruct u as [[| |] l] => //; cbv[Universe.to_csort]. eexists; eauto.
 Qed.
 
-Lemma val_is_prop_false s v n :
-  Sort.to_csort v s = sType n -> Sort.is_prop s = false.
+Lemma val_is_prop_false u v n :
+  Universe.to_csort v u = Universe.mk sType n -> Universe.is_prop u = false.
+Proof. destruct u as [[| |] l] => //. Qed.
+
+Lemma get_is_level_correct u l :
+  Universe.get_is_level u = Some l -> u = Universe.mk sType (UnivLvl.make' l).
 Proof.
-  destruct s => //.
+  intro H; destruct u as [[| |] l'] => //.
+  f_equal; now apply ulvl_get_is_level_correct.
 Qed.
 
-Lemma get_is_level_correct s l :
-  Sort.get_is_level s = Some l -> s = sType (Universe.make' l).
-Proof.
-  intro H; destruct s => //=.
-  f_equal; now apply universe_get_is_level_correct.
-Qed.
-
-Lemma eqb_true_iff (s s' : sort) :
-  eqb s s' <-> s = s'.
+Lemma eqb_true_iff (u u' : Universe.t) :
+  eqb u u' <-> u = u'.
 Proof.
   split. apply /eqb_spec. eapply introP. apply /eqb_spec.
 Qed.
 
-Lemma sup_comm x1 x2 :
-  Sort.sup x1 x2 = Sort.sup x2 x1.
+Lemma sup_comm u1 u2 :
+  Universe.sup u1 u2 = Universe.sup u2 u1.
 Proof.
-  destruct x1,x2;auto.
-  cbn;apply f_equal;apply sup0_comm.
+  destruct u1 as [[| |] l1], u2 as [[| |] l2]; cbnr.
+  all: f_equal; apply sup0_comm.
 Qed.
 
-Lemma is_not_prop_and_is_not_sprop {univ} (s : Sort.t_ univ) :
-  Sort.is_prop s = false -> Sort.is_sprop s = false ->
-  ∑ s', s = sType s'.
+Lemma is_not_prop_and_is_not_sprop {univ} (u : Universe.t_ Sort.t univ) :
+  Universe.is_prop u = false -> Universe.is_sprop u = false ->
+  ∑ l, u = Universe.mk sType l.
 Proof.
   intros Hp Hsp.
-  destruct s => //. now eexists.
+  destruct u as [[| |] l] => //. now eexists.
 Qed.
 
-Lemma is_prop_sort_sup x1 x2 :
-  Sort.is_prop (Sort.sup x1 x2)
-  -> Sort.is_prop x2 \/ Sort.is_sprop x2 .
-Proof. destruct x1,x2;auto. Qed.
+Lemma is_prop_sort_sup u1 u2 :
+  Universe.is_prop (Universe.sup u1 u2)
+  -> Universe.is_prop u2 \/ Universe.is_sprop u2 .
+Proof. destruct u1 as [[| |] l1], u2 as [[| |] l2]; auto. Qed.
 
-Lemma is_prop_sort_sup' x1 x2 :
-  Sort.is_prop (Sort.sup x1 x2)
-  -> Sort.is_prop x1 \/ Sort.is_sprop x1 .
-Proof. destruct x1,x2;auto. Qed.
+Lemma is_prop_sort_sup' u1 u2 :
+  Universe.is_prop (Universe.sup u1 u2)
+  -> Universe.is_prop u1 \/ Universe.is_sprop u1 .
+Proof. destruct u1 as [[| |] l1], u2 as [[| |] l2]; auto. Qed.
 
-Lemma is_prop_or_sprop_sort_sup x1 x2 :
-  Sort.is_sprop (Sort.sup x1 x2) -> Sort.is_sprop x2.
-Proof. destruct x1,x2;auto. Qed.
+Lemma is_prop_or_sprop_sort_sup u1 u2 :
+  Universe.is_sprop (Universe.sup u1 u2) -> Universe.is_sprop u2.
+Proof. destruct u1 as [[| |] l1], u2 as [[| |] l2]; auto. Qed.
 
-Lemma is_prop_sort_sup_prop x1 x2 :
-  Sort.is_prop x1 && Sort.is_prop x2 ->
-  Sort.is_prop (Sort.sup x1 x2).
-Proof. destruct x1,x2;auto. Qed.
+Lemma is_prop_sort_sup_prop u1 u2 :
+  Universe.is_prop u1 && Universe.is_prop u2 ->
+  Universe.is_prop (Universe.sup u1 u2).
+Proof. destruct u1 as [[| |] l1], u2 as [[| |] l2]; auto. Qed.
 
-Lemma is_prop_or_sprop_sort_sup_prop x1 x2 :
-  Sort.is_sprop x1 && Sort.is_sprop x2 ->
-  Sort.is_sprop (Sort.sup x1 x2).
-Proof. destruct x1,x2;auto. Qed.
+Lemma is_prop_or_sprop_sort_sup_prop u1 u2 :
+  Universe.is_sprop u1 && Universe.is_sprop u2 ->
+  Universe.is_sprop (Universe.sup u1 u2).
+Proof. destruct u1 as [[| |] l1], u2 as [[| |] l2]; auto. Qed.
 
-Lemma is_prop_sup s s' :
-  Sort.is_prop (Sort.sup s s') ->
-  Sort.is_propositional s /\ Sort.is_propositional s'.
-Proof. destruct s, s'; auto. Qed.
+Lemma is_prop_sup u1 u2 :
+  Universe.is_prop (Universe.sup u1 u2) ->
+  Universe.is_propositional u1 /\ Universe.is_propositional u2.
+Proof. destruct u1 as [[| |] l1], u2 as [[| |] l2]; auto. Qed.
 
-Lemma is_sprop_sup_iff s s' :
-  Sort.is_sprop (Sort.sup s s') <->
-  (Sort.is_sprop s /\ Sort.is_sprop s').
-Proof. split; destruct s, s' => //=; intuition. Qed.
+Lemma is_sprop_sup_iff u1 u2 :
+  Universe.is_sprop (Universe.sup u1 u2) <->
+  (Universe.is_sprop u1 /\ Universe.is_sprop u2).
+Proof. split; destruct u1 as [[| |] l1], u2 as [[| |] l2] => //=; intuition. Qed.
 
-Lemma is_type_sup_r s1 s2 :
-  Sort.is_type_sort s2 ->
-  Sort.is_type_sort (Sort.sup s1 s2).
-Proof. destruct s2; try absurd; destruct s1; cbnr; intros; absurd. Qed.
+Lemma is_type_sup_r u1 u2 :
+  Universe.is_type_sort u2 ->
+  Universe.is_type_sort (Universe.sup u1 u2).
+Proof. destruct u2 as [[| |] l2]; try absurd; destruct u1 as [[| |] l1]; cbnr; intros; absurd. Qed.
 
-Lemma is_prop_sort_prod x2 x3 :
-  Sort.is_prop (Sort.sort_of_product x2 x3)
-  -> Sort.is_prop x3.
+Lemma is_prop_univ_prod u1 u2 :
+  Universe.is_prop (Universe.univ_of_product u1 u2)
+  -> Universe.is_prop u2.
 Proof.
-  unfold Sort.sort_of_product.
-  destruct x3;cbn;auto.
-  intros;simpl in *;destruct x2;auto.
+  unfold Universe.univ_of_product.
+  destruct u2 as [[| |] l2]; cbn; auto.
+  intros; simpl in *; destruct u1 as [[| |] l1]; auto.
 Qed.
 
-Lemma is_sprop_sort_prod x2 x3 :
-  Sort.is_sprop (Sort.sort_of_product x2 x3)
-  -> Sort.is_sprop x3.
+Lemma is_sprop_univ_prod u1 u2 :
+  Universe.is_sprop (Universe.univ_of_product u1 u2)
+  -> Universe.is_sprop u2.
 Proof.
-  unfold Sort.sort_of_product.
-  destruct x3;cbn;auto.
-  intros;simpl in *;destruct x2;auto.
+  unfold Universe.univ_of_product.
+  destruct u2 as [[| |] l2]; cbn; auto.
+  intros; simpl in *; destruct u1 as [[| |] l1]; auto.
 Qed.
 
-
-
-Section SortCompare.
+Section UnivCompare.
   Context {cf}.
-  Definition leq_sort_n_ {univ} (leq_universe_n : Z -> univ -> univ -> Prop) n s s' : Prop :=
-    match s, s' with
+  Definition leq_univ_n_ {univ} (leq_universe_n : Z -> univ -> univ -> Prop) n u u' : Prop :=
+    match usort u, usort u' with
     | sProp,   sProp
     | sSProp,  sSProp => (n = 0)%Z
-    | sType u, sType u' => leq_universe_n n u u'
-    | sProp,   sType u => prop_sub_type
+    | sType, sType => leq_universe_n n (ulvl u) (ulvl u')
+    | sProp,   sType => prop_sub_type
     | _, _ => False
     end.
 
-  Definition leq_sort_n n φ := leq_sort_n_ (fun n => leq_universe_n n φ) n.
-  Definition lt_sort := leq_sort_n 1.
-  Definition leq_sort := leq_sort_n 0.
+  Definition leq_univ_n n φ := leq_univ_n_ (fun n => leq_ulvl_n n φ) n.
+  Definition lt_univ := leq_univ_n 1.
+  Definition leq_univ := leq_univ_n 0.
 
-  Definition leqb_sort_n_ {univ} (leqb_universe_n : bool -> univ -> univ -> bool) b s s' : bool :=
-    match s, s' with
+  Definition leqb_univ_n_ {univ} (leqb_universe_n : bool -> univ -> univ -> bool) b u u' : bool :=
+    match usort u, usort u' with
     | sProp,   sProp
     | sSProp,  sSProp => negb b
-    | sType u, sType u' => leqb_universe_n b u u'
-    | sProp,   sType u => prop_sub_type
+    | sType, sType => leqb_universe_n b (ulvl u) (ulvl u')
+    | sProp,   sType => prop_sub_type
     | _, _ => false
     end.
 
-  Definition eq_sort_ {univ} (eq_universe : univ -> univ -> Prop) s s' : Prop :=
-    match s, s' with
+  Definition eq_univ_ {univ} (eq_universe : univ -> univ -> Prop) u u' : Prop :=
+    match usort u, usort u' with
     | sProp,   sProp
     | sSProp,  sSProp => True
-    | sType u, sType u' => eq_universe u u'
+    | sType, sType => eq_universe (ulvl u) (ulvl u')
     | _, _ => False
     end.
 
-  Definition eq_sort φ := eq_sort_ (eq_universe φ).
+  Definition eq_univ φ := eq_univ_ (eq_ulvl φ).
 
-  Definition eqb_sort_ {univ} (eqb_universe : univ -> univ -> bool) s s' : bool :=
-    match s, s' with
+  Definition eqb_univ_ {univ} (eqb_universe : univ -> univ -> bool) u u' : bool :=
+    match usort u, usort u' with
     | sProp,   sProp
     | sSProp,  sSProp => true
-    | sType u, sType u' => eqb_universe u u'
+    | sType, sType => eqb_universe (ulvl u) (ulvl u')
     | _, _ => false
     end.
 
-  Definition compare_sort φ (pb : conv_pb) :=
+  Definition compare_univ φ (pb : conv_pb) :=
     match pb with
-    | Conv => eq_sort φ
-    | Cumul => leq_sort φ
+    | Conv => eq_univ φ
+    | Cumul => leq_univ φ
     end.
 
-  Lemma leq_sort_leq_sort_n (φ : ConstraintSet.t) s s' :
-    leq_sort φ s s' <-> leq_sort_n 0 φ s s'.
-  Proof using Type. intros. reflexivity. Qed.
+  Lemma leq_univ_leq_univ_n (φ : ConstraintSet.t) u u' :
+    leq_univ φ u u' <-> leq_univ_n 0 φ u u'.
+  Proof. intros. reflexivity. Qed.
 
-  Lemma compare_sort_type φ pb u u' :
-    compare_sort φ pb (sType u) (sType u') = compare_universe φ pb u u'.
+  Lemma compare_univ_type φ pb l l' :
+    compare_univ φ pb (Universe.mk sType l) (Universe.mk sType l') = compare_ulvl φ pb l l'.
   Proof. now destruct pb. Qed.
 
   Section GeneralLemmas.
     Context {univ} {leq_universe_n : Z -> univ -> univ -> Prop} {eq_universe : univ -> univ -> Prop}.
 
-    Let leq_sort_n := leq_sort_n_ leq_universe_n.
-    Let lt_sort := leq_sort_n_ leq_universe_n 1.
-    Let leq_sort := leq_sort_n_ leq_universe_n 0.
-    Let eq_sort := eq_sort_ eq_universe.
-    Notation "x <_ n  y" := (leq_sort_n n x y) (at level 10, n name).
-    Notation "x < y" := (lt_sort x y).
-    Notation "x <= y" := (leq_sort x y).
+    Let leq_univ_n := leq_univ_n_ leq_universe_n.
+    Let lt_univ := leq_univ_n_ leq_universe_n 1.
+    Let leq_univ := leq_univ_n_ leq_universe_n 0.
+    Let eq_univ := eq_univ_ eq_universe.
+    Notation "x <_ n  y" := (leq_univ_n n x y) (at level 10, n name).
+    Notation "x < y" := (lt_univ x y).
+    Notation "x <= y" := (leq_univ x y).
 
+    Lemma univ_le_prop_inv u l : u <= Universe.mk sProp l -> usort u = sProp.
+    Proof using Type. destruct u as [[| |] l'] => //. Qed.
 
-    Lemma sort_le_prop_inv s : s <= sProp -> s = sProp.
-    Proof using Type. destruct s => //. Qed.
+    Lemma univ_le_sprop_inv u l : u <= Universe.mk sSProp l -> usort u = sSProp.
+    Proof using Type. destruct u as [[| |] l'] => //. Qed.
 
-    Lemma sort_le_sprop_inv s : s <= sSProp -> s = sSProp.
-    Proof using Type. destruct s => //. Qed.
-
-    Lemma sort_prop_le_inv s : sProp <= s ->
-      (s = sProp \/ (prop_sub_type /\ exists n, s = sType n)).
+    Lemma univ_prop_le_inv u l : Universe.mk sProp l <= u ->
+      (usort u = sProp \/ (prop_sub_type /\ exists n, u = Universe.mk sType n)).
     Proof using Type.
-      destruct s => //= Hle.
+      destruct u as [[| |] l'] => //= Hle.
       - now left.
       - right; split => //; now eexists.
     Qed.
 
-    Lemma sort_sprop_le_inv s : sSProp <= s -> s = sSProp.
-    Proof using Type. destruct s => //. Qed.
+    Lemma univ_sprop_le_inv u l : Universe.mk sSProp l <= u -> usort u = sSProp.
+    Proof using Type. destruct u as [[| |] l'] => //. Qed.
 
-    Global Instance leq_sort_refl `{Reflexive univ (leq_universe_n 0)} : Reflexive leq_sort.
-    Proof using Type. intros []; cbnr. Qed.
+    Global Instance leq_univ_refl `{Reflexive univ (leq_universe_n 0)} : Reflexive leq_univ.
+    Proof using Type. intros [[| |] l]; cbnr. Qed.
 
-    Global Instance eq_sort_refl `{Reflexive univ eq_universe} : Reflexive eq_sort.
-    Proof using Type. intros []; cbnr. Qed.
+    Global Instance eq_univ_refl `{Reflexive univ eq_universe} : Reflexive eq_univ.
+    Proof using Type. intros [[| |] l]; cbnr. Qed.
 
-    Global Instance eq_sort_sym `{Symmetric univ eq_universe} : Symmetric eq_sort.
-    Proof using Type. intros [] [] => //=. apply H. Qed.
+    Global Instance eq_univ_sym `{Symmetric univ eq_universe} : Symmetric eq_univ.
+    Proof using Type. intros [[| |] l] [[| |] l'] => //=. apply H. Qed.
 
-    Global Instance leq_sort_n_trans n `{Transitive univ (leq_universe_n n)} : Transitive (leq_sort_n n).
+    Global Instance leq_univ_n_trans n `{Transitive univ (leq_universe_n n)} : Transitive (leq_univ_n n).
     Proof using Type.
-      intros [] [] [] => //=. apply H.
+      intros [[| |] l1] [[| |] l2] [[| |] l3] => //=. apply H.
     Qed.
 
-    Global Instance leq_sort_trans `{Transitive univ (leq_universe_n 0)} : Transitive leq_sort.
-    Proof using Type. apply (leq_sort_n_trans 0). Qed.
+    Global Instance leq_univ_trans `{Transitive univ (leq_universe_n 0)} : Transitive leq_univ.
+    Proof using Type. apply (leq_univ_n_trans 0). Qed.
 
-    Global Instance lt_sort_trans `{Transitive univ (leq_universe_n 1)} : Transitive lt_sort.
-    Proof using Type. apply (leq_sort_n_trans 1). Qed.
+    Global Instance lt_univ_trans `{Transitive univ (leq_universe_n 1)} : Transitive lt_univ.
+    Proof using Type. apply (leq_univ_n_trans 1). Qed.
 
-    Global Instance eq_sort_trans `{Transitive univ eq_universe} : Transitive eq_sort.
+    Global Instance eq_univ_trans `{Transitive univ eq_universe} : Transitive eq_univ.
     Proof using Type.
-      intros [] [] [] => //=. apply H.
+      intros [[| |] l1] [[| |] l2] [[| |] l3] => //=. apply H.
     Qed.
 
-    Global Instance leq_sort_preorder `{PreOrder univ (leq_universe_n 0)} : PreOrder leq_sort :=
+    Global Instance leq_univ_preorder `{PreOrder univ (leq_universe_n 0)} : PreOrder leq_univ :=
       Build_PreOrder _ _ _.
 
     (* Can't be a global instance since it can lead to infinite search *)
-    Lemma lt_sort_irrefl : Irreflexive (leq_universe_n 1) -> Irreflexive lt_sort.
+    Lemma lt_univ_irrefl : Irreflexive (leq_universe_n 1) -> Irreflexive lt_univ.
     Proof using Type.
-      intros H []; unfold complement; cbnr. 1,2: lia. apply H.
+      intros H [[| |] l]; unfold complement; cbnr. 1,2: lia. apply H.
     Qed.
 
-    Global Instance lt_sort_str_order `{StrictOrder univ (leq_universe_n 1)} : StrictOrder lt_sort :=
-      Build_StrictOrder _ (lt_sort_irrefl _) _.
+    Global Instance lt_univ_str_order `{StrictOrder univ (leq_universe_n 1)} : StrictOrder lt_univ :=
+      Build_StrictOrder _ (lt_univ_irrefl _) _.
 
-    Global Instance eq_leq_sort `{subrelation univ eq_universe (leq_universe_n 0)}: subrelation eq_sort leq_sort.
+    Global Instance eq_leq_univ `{subrelation univ eq_universe (leq_universe_n 0)}: subrelation eq_univ leq_univ.
     Proof using Type.
-      intros [] [] => //=. apply H.
+      intros [[| |] l1] [[| |] l2] => //=. apply H.
     Qed.
 
-    Global Instance eq_sort_equivalence `{Equivalence univ eq_universe} : Equivalence eq_sort := Build_Equivalence _ _ _ _.
+    Global Instance eq_univ_equivalence `{Equivalence univ eq_universe} : Equivalence eq_univ := Build_Equivalence _ _ _ _.
 
-    Global Instance leq_sort_antisym `{Antisymmetric _ eq_universe (leq_universe_n 0)} : Antisymmetric _ eq_sort leq_sort.
+    Global Instance leq_univ_antisym `{Antisymmetric _ eq_universe (leq_universe_n 0)} : Antisymmetric _ eq_univ leq_univ.
     Proof using Type.
-      intros [] [] => //=. apply H.
+      intros [[| |] l1] [[| |] l2] => //=. apply H.
     Qed.
 
-    Global Instance leq_sort_partial_order `{PartialOrder _ eq_universe (leq_universe_n 0)}: PartialOrder eq_sort leq_sort.
+    Global Instance leq_univ_partial_order `{PartialOrder _ eq_universe (leq_universe_n 0)}: PartialOrder eq_univ leq_univ.
     Proof.
       assert (subrelation eq_universe (leq_universe_n 0)).
       { intros u u' Hu. specialize (H u u'); cbn in H. apply H in Hu. apply Hu. }
@@ -1974,172 +509,169 @@ Section SortCompare.
       { intros u u' Hu. specialize (H u u'); cbn in H. apply H in Hu. apply Hu. }
       intros s s'. split.
       - intro Heq. split.
-        + now eapply eq_leq_sort.
-        + now eapply eq_leq_sort.
-      - intros [Hle Hge]. now eapply leq_sort_antisym.
+        + now eapply eq_leq_univ.
+        + now eapply eq_leq_univ.
+      - intros [Hle Hge]. now eapply leq_univ_antisym.
     Qed.
 
   End GeneralLemmas.
 
-
   (** Universes with linear hierarchy *)
-  Definition concrete_sort := Sort.t_ nat.
+  Definition concrete_univ := Universe.t_ Sort.t nat.
 
   (** u + n <= u' *)
-  Definition leq_csort_n : Z -> concrete_sort -> concrete_sort -> Prop :=
-    leq_sort_n_ (fun n u u' => (Z.of_nat u <= Z.of_nat u' - n)%Z).
+  Definition leq_cuniv_n : Z -> concrete_univ -> concrete_univ -> Prop :=
+    leq_univ_n_ (fun n u u' => (Z.of_nat u <= Z.of_nat u' - n)%Z).
 
-  Definition leq_csort := leq_csort_n 0.
-  Definition lt_csort := leq_csort_n 1.
+  Definition leq_cuniv := leq_cuniv_n 0.
+  Definition lt_cuniv := leq_cuniv_n 1.
 
-  Notation "x <_ n  y" := (leq_csort_n n x y) (at level 10, n name) : univ_scope.
-  Notation "x < y" := (lt_csort x y) : univ_scope.
-  Notation "x <= y" := (leq_csort x y) : univ_scope.
+  Notation "x <_ n  y" := (leq_univ_n n x y) (at level 10, n name) : univ_scope.
+  Notation "x < y" := (lt_cuniv x y) : univ_scope.
+  Notation "x <= y" := (leq_cuniv x y) : univ_scope.
 
-  Definition is_propositional_or_set s := match s with sSProp | sProp | sType 0 => true | _ => false end.
+  Definition is_propositional_or_set u :=
+    match usort u with
+	| sSProp | sProp => true
+	| sType => eqb (ulvl u) 0
+	end.
 
-  Lemma csort_sup_comm s s' : Sort.csup s s' = Sort.csup s' s.
-  Proof using Type. destruct s, s' => //=. f_equal; lia. Qed.
-
-  Lemma csort_sup_not_uproplevel s s' :
-    ~ Sort.is_propositional s -> ∑ n, Sort.csup s s' = sType n.
+  Lemma cuniv_sup_comm u u' : Universe.csup u u' = Universe.csup u' u.
   Proof using Type.
-    destruct s => //=.
-    destruct s'; now eexists.
+    destruct u as [[| |] n], u' as [[| |] m] => //=; cbnr; f_equal; lia.
   Qed.
 
-  Lemma csort_sup_mon s s' v v' : (s <= s')%u -> (sType v <= sType v')%u ->
-    (Sort.csup s (sType v) <= Sort.csup s' (sType v'))%u.
+  Lemma cuniv_sup_not_uproplevel u u' :
+    ~ Universe.is_propositional u -> ∑ n, Universe.csup u u' = Universe.mk sType n.
   Proof using Type.
-    destruct s, s' => //=; intros Hle Hle';
-    lia.
+    destruct u as [[| |] n] => //=.
+    destruct u' as [[| |] m]; now eexists.
   Qed.
 
-  Lemma leq_csort_of_product_mon u u' v v' :
+  Lemma cuniv_sup_mon u0 u' l l' : (u0 <= u')%u -> (Universe.mk sType l <= Universe.mk sType l')%u ->
+    (Universe.csup u0 (Universe.mk sType l) <= Universe.csup u' (Universe.mk sType l'))%u.
+  Proof using Type.
+    destruct u0 as [[| |] l0], u' as [[| |] l0'] => //=; cbn; intros Hle Hle'; lia.
+  Qed.
+
+  Lemma leq_cuniv_of_product_mon u u' v v' :
     (u <= u')%u ->
     (v <= v')%u ->
-    (Sort.csort_of_product u v <= Sort.csort_of_product u' v')%u.
+    (Universe.cuniv_of_product u v <= Universe.cuniv_of_product u' v')%u.
   Proof using Type.
     intros Hle1 Hle2.
-    destruct v, v'; cbn in Hle2 |- *; auto.
-    - destruct u'; cbn; assumption.
-    - apply csort_sup_mon; assumption.
+    destruct v as [[| |] l], v' as [[| |] l']; cbn in Hle2 |- *; auto.
+    - destruct u' as [[| |] l'']; cbn; assumption.
+    - apply cuniv_sup_mon; assumption.
   Qed.
 
-  Lemma impredicative_csort_product {univ} {univ_sup} {l u} :
-    Sort.is_propositional u ->
-    Sort.sort_of_product_ (univ := univ) univ_sup l u = u.
-  Proof using Type. now destruct u. Qed.
+  Lemma impredicative_cuniv_product {ulvl} {type0} {univ_sup} {l u} :
+    Universe.is_propositional u ->
+    Universe.univ_of_product_ (ulvl := ulvl) type0 univ_sup l u = u.
+  Proof using Type. now destruct u as [[| |] l0]. Qed.
 
-  Lemma leq_sort_sup_l φ u1 s2 :
-    let s1 := sType u1 in
-    leq_sort φ s1 (Sort.sup s1 s2).
+  Lemma leq_univ_sup_l φ u1 s2 :
+    let s1 := Universe.mk sType u1 in
+    leq_univ φ s1 (Universe.sup s1 s2).
   Proof using Type.
-    destruct s2 as [| | u2]; cbnr.
-    apply leq_universe_sup_l.
+    destruct s2 as [[| |] u2]; cbnr.
+    apply leq_ulvl_sup_l.
   Qed.
 
-  Lemma leq_sort_sup_r φ s1 u2 :
-    let s2 := sType u2 in
-    leq_sort φ s2 (Sort.sup s1 s2).
+  Lemma leq_univ_sup_r φ s1 u2 :
+    let s2 := Universe.mk sType u2 in
+    leq_univ φ s2 (Universe.sup s1 s2).
   Proof using Type.
-    destruct s1 as [| | u1]; cbnr.
-    apply leq_universe_sup_r.
+    destruct s1 as [[| |] u1]; cbnr.
+    apply leq_ulvl_sup_r.
   Qed.
 
-  Lemma leq_sort_product φ (s1 s2 : Sort.t)
-    : leq_sort φ s2 (Sort.sort_of_product s1 s2).
+  Lemma leq_univ_product φ (s1 s2 : Universe.t)
+    : leq_univ φ s2 (Universe.univ_of_product s1 s2).
   Proof using Type.
-    destruct s2 as [| | u2] => //.
-    apply leq_sort_sup_r.
+    destruct s2 as [[| |] u2] => //.
+    apply leq_univ_sup_r.
   Qed.
-  (* Rk: [leq_universe φ s1 (sort_of_product s1 s2)] does not hold due to
+  (* Rk: [leq_universe φ s1 (univ_of_product s1 s2)] does not hold due to
       impredicativity. *)
 
-
-  Global Instance lt_sort_irrefl' {c: check_univs} φ (H: consistent φ) : Irreflexive (lt_sort φ).
+  Global Instance lt_univ_irrefl' {c: check_univs} φ (H: consistent φ) : Irreflexive (lt_univ φ).
   Proof.
-    unshelve eapply lt_sort_irrefl.
-    now unshelve eapply lt_universe_irrefl.
+    unshelve eapply lt_univ_irrefl.
+    now unshelve eapply lt_ulvl_irrefl.
   Qed.
 
-  Global Instance lt_sort_str_order' {c: check_univs} φ (H: consistent φ) : StrictOrder (lt_sort φ).
+  Global Instance lt_univ_str_order' {c: check_univs} φ (H: consistent φ) : StrictOrder (lt_univ φ).
   Proof using Type.
-    unshelve eapply lt_sort_str_order.
-    now unshelve eapply lt_universe_str_order.
+    unshelve eapply lt_univ_str_order.
+    now unshelve eapply lt_ulvl_str_order.
   Qed.
 
-  Global Instance compare_sort_subrel φ pb : subrelation (eq_sort φ) (compare_sort φ pb).
-  Proof using Type.
-    destruct pb; tc.
-  Qed.
-
-  Global Instance compare_sort_refl φ pb : Reflexive (compare_sort φ pb).
+  Global Instance compare_univ_subrel φ pb : subrelation (eq_univ φ) (compare_univ φ pb).
   Proof using Type.
     destruct pb; tc.
   Qed.
 
-  Global Instance compare_sort_trans φ pb : Transitive (compare_sort φ pb).
+  Global Instance compare_sort_refl φ pb : Reflexive (compare_univ φ pb).
   Proof using Type.
     destruct pb; tc.
   Qed.
 
-  Global Instance compare_sort_preorder φ pb : PreOrder (compare_sort φ pb).
+  Global Instance compare_sort_trans φ pb : Transitive (compare_univ φ pb).
   Proof using Type.
     destruct pb; tc.
   Qed.
 
-  Definition eq_leq_sort' φ leq_universe eq_universe Hsub u u'
-    := @eq_leq_sort φ leq_universe eq_universe Hsub u u'.
-  Definition leq_sort_refl' φ leq_universe leq_refl u
-    := @leq_sort_refl φ leq_universe leq_refl u.
+  Global Instance compare_sort_preorder φ pb : PreOrder (compare_univ φ pb).
+  Proof using Type.
+    destruct pb; tc.
+  Qed.
 
-  Hint Resolve eq_leq_universe' leq_universe_refl' : core.
+  Definition eq_leq_univ' φ leq_universe eq_universe Hsub u u'
+    := @eq_leq_univ φ leq_universe eq_universe Hsub u u'.
+  Definition leq_univ_refl' φ leq_universe leq_refl u
+    := @leq_univ_refl φ leq_universe leq_refl u.
 
+  Hint Resolve eq_leq_ulvl' leq_ulvl_refl' : core.
 
-  Lemma cmp_sort_subset φ φ' pb t u
+  Lemma cmp_univ_subset φ φ' pb t u
     : ConstraintSet.Subset φ φ'
-      -> compare_sort φ pb t u -> compare_sort φ' pb t u.
+      -> compare_univ φ pb t u -> compare_univ φ' pb t u.
   Proof using Type.
     intros Hctrs.
-    destruct pb, t, u; cbnr; trivial.
-    all: intros H; unfold_univ_rel;
+    destruct pb, t as [[| |] l], u as [[| |] l']; cbnr; trivial.
+    all: intros H; unfold_ulvl_rel;
     apply H.
     all: eapply satisfies_subset; eauto.
   Qed.
 
-  Lemma eq_sort_subset ctrs ctrs' t u
+  Lemma eq_univ_subset ctrs ctrs' t u
     : ConstraintSet.Subset ctrs ctrs'
-      -> eq_sort ctrs t u -> eq_sort ctrs' t u.
-  Proof using Type. apply cmp_sort_subset with (pb := Conv). Qed.
+      -> eq_univ ctrs t u -> eq_univ ctrs' t u.
+  Proof using Type. apply cmp_univ_subset with (pb := Conv). Qed.
 
-  Lemma leq_sort_subset ctrs ctrs' t u
+  Lemma leq_univ_subset ctrs ctrs' t u
     : ConstraintSet.Subset ctrs ctrs'
-      -> leq_sort ctrs t u -> leq_sort ctrs' t u.
-  Proof using Type. apply cmp_sort_subset with (pb := Cumul). Qed.
-End SortCompare.
+      -> leq_univ ctrs t u -> leq_univ ctrs' t u.
+  Proof using Type. apply cmp_univ_subset with (pb := Cumul). Qed.
+End UnivCompare.
 
-
-
-Definition relevance_of_family (s : Sort.family) :=
+Definition relevance_of_family (s : Sort.t) :=
   match s with
-  | Sort.fSProp => Irrelevant
+  | sSProp => Irrelevant
   | _ => Relevant
   end.
 
 #[global] Opaque relevance_of_family.
 
-Notation rel_of_Type := (relevance_of_family Sort.fType).
-Notation relevance_of_sort s := (relevance_of_family (Sort.to_family s)).
+Notation rel_of_Type := (relevance_of_family sType).
+Notation relevance_of_univ s := (relevance_of_family (Universe.to_family s)).
 
-Notation isSortRel s rel := (relevance_of_sort s = rel).
-Notation isSortRelOpt s relopt :=
-  (option_default (fun rel => isSortRel s rel) relopt True).
-
-
+Notation isUnivRel s rel := (relevance_of_univ s = rel).
+Notation isUnivRelOpt s relopt :=
+  (option_default (fun rel => isUnivRel s rel) relopt True).
 
 (** Elimination restriction *)
-
 
 (** This inductive classifies which eliminations are allowed for inductive types
   in various sorts. *)
@@ -2150,28 +682,27 @@ Inductive allowed_eliminations : Set :=
   | IntoAny.
 Derive NoConfusion EqDec for allowed_eliminations.
 
-
-Definition is_allowed_elimination_cuniv (allowed : allowed_eliminations) : concrete_sort -> bool :=
+Definition is_allowed_elimination_cuniv (allowed : allowed_eliminations) : concrete_univ -> bool :=
   match allowed with
-  | IntoSProp => Sort.is_sprop
-  | IntoPropSProp => Sort.is_propositional
+  | IntoSProp => Universe.is_sprop
+  | IntoPropSProp => Universe.is_propositional
   | IntoSetPropSProp => is_propositional_or_set
   | IntoAny => fun _ => true
   end.
 
-Definition is_lSet {cf} φ s := eq_sort φ s Sort.type0.
+Definition is_lSet {cf} φ s := eq_univ φ s Universe.type0.
   (* Unfolded definition :
   match s with
-  | Sort.sType u =>
+  | Universe.sType u =>
     if check_univs then forall v, satisfies v φ -> val v u = 0 else true
   | _ => false
   end. *)
 
-Definition is_allowed_elimination {cf} φ allowed : Sort.t -> Prop :=
+Definition is_allowed_elimination {cf} φ allowed : Universe.t -> Prop :=
   match allowed with
-  | IntoSProp => Sort.is_sprop
-  | IntoPropSProp => Sort.is_propositional
-  | IntoSetPropSProp => fun s => Sort.is_propositional s \/ is_lSet φ s
+  | IntoSProp => Universe.is_sprop
+  | IntoPropSProp => Universe.is_propositional
+  | IntoSetPropSProp => fun s => Universe.is_propositional s \/ is_lSet φ s
   | IntoAny => fun s => true
   end.
 
@@ -2190,18 +721,18 @@ Lemma allowed_eliminations_subset_impl {cf} φ a a' s
     is_allowed_elimination φ a s -> is_allowed_elimination φ a' s.
 Proof using Type.
   destruct a, a'; cbnr; trivial;
-  destruct s; cbnr; trivial;
+  destruct s as [[| |] l]; cbnr; trivial;
   intros H1 H2; try absurd; constructor; trivial.
 Qed.
 
 Lemma is_allowed_elimination_monotone `{cf : checker_flags} Σ s1 s2 a :
-  leq_sort Σ s1 s2 -> is_allowed_elimination Σ a s2 -> is_allowed_elimination Σ a s1.
+  leq_univ Σ s1 s2 -> is_allowed_elimination Σ a s2 -> is_allowed_elimination Σ a s1.
 Proof.
-  destruct a, s2 as [| |u2], s1 as [| |u1] => //=. 1: now left.
+  destruct a, s2 as [[| |] u2], s1 as [[| |] u1] => //=. 1: now left.
   intros Hle [H|]; right => //.
-  unfold_univ_rel.
-  cbn in H.
-  lia.
+  unfold_ulvl_rel; cbn in H, Hle |- *; rewrite H in Hle;
+  unfold eq_ulvl; unfold leq_ulvl_n, leq0_ulvl_n in Hle; destruct check_univs; auto.
+  all: intros v hsat; specialize (Hle v hsat); cbn in *; lia.
 Qed.
 
 Section UnivCF2.
@@ -2217,42 +748,42 @@ Section UnivCF2.
 
   Lemma cmp_universe_config_impl ctrs pb t u
     : config.impl cf1 cf2
-      -> @compare_universe cf1 ctrs pb t u -> @compare_universe cf2 ctrs pb t u.
+      -> @compare_ulvl cf1 ctrs pb t u -> @compare_ulvl cf2 ctrs pb t u.
   Proof using Type.
-    unfold config.impl, compare_universe, leq_universe, eq_universe, leq_universe_n, is_true.
+    unfold config.impl, compare_ulvl, leq_ulvl, eq_ulvl, leq_ulvl_n, is_true.
     destruct pb; do 2 destruct check_univs => //=.
   Qed.
 
   Lemma eq_universe_config_impl ctrs t u
     : config.impl cf1 cf2
-      -> @eq_universe cf1 ctrs t u -> @eq_universe cf2 ctrs t u.
+      -> @eq_ulvl cf1 ctrs t u -> @eq_ulvl cf2 ctrs t u.
   Proof using Type. apply cmp_universe_config_impl with (pb := Conv). Qed.
 
   Lemma leq_universe_config_impl ctrs t u
     : config.impl cf1 cf2
-      -> @leq_universe cf1 ctrs t u -> @leq_universe cf2 ctrs t u.
+      -> @leq_ulvl cf1 ctrs t u -> @leq_ulvl cf2 ctrs t u.
   Proof using Type. apply cmp_universe_config_impl with (pb := Cumul). Qed.
 
-  Lemma cmp_sort_config_impl ctrs pb t u
+  Lemma cmp_univ_config_impl ctrs pb t u
     : config.impl cf1 cf2
-      -> @compare_sort cf1 ctrs pb t u -> @compare_sort cf2 ctrs pb t u.
+      -> @compare_univ cf1 ctrs pb t u -> @compare_univ cf2 ctrs pb t u.
   Proof using Type.
-    unfold compare_sort, leq_sort, eq_sort, eq_sort_, leq_sort_n, leq_sort_n_, is_true.
-    destruct pb, t, u => //=.
+    unfold compare_univ, leq_univ, eq_univ, eq_univ_, leq_univ_n, leq_univ_n_, is_true.
+    destruct pb, t as [[| |] t1], u as [[| |] u1] => //=.
     - apply eq_universe_config_impl.
     - unfold config.impl. do 2 destruct check_univs, prop_sub_type; cbn => //=.
     - apply leq_universe_config_impl.
   Qed.
 
-  Lemma eq_sort_config_impl ctrs t u
+  Lemma eq_univ_config_impl ctrs t u
     : config.impl cf1 cf2
-      -> @eq_sort cf1 ctrs t u -> @eq_sort cf2 ctrs t u.
-  Proof using Type. apply cmp_sort_config_impl with (pb := Conv). Qed.
+      -> @eq_univ cf1 ctrs t u -> @eq_univ cf2 ctrs t u.
+  Proof using Type. apply cmp_univ_config_impl with (pb := Conv). Qed.
 
-  Lemma leq_sort_config_impl ctrs t u
+  Lemma leq_univ_config_impl ctrs t u
     : config.impl cf1 cf2
-      -> @leq_sort cf1 ctrs t u -> @leq_sort cf2 ctrs t u.
-  Proof using Type. apply cmp_sort_config_impl with (pb := Cumul). Qed.
+      -> @leq_univ cf1 ctrs t u -> @leq_univ cf2 ctrs t u.
+  Proof using Type. apply cmp_univ_config_impl with (pb := Cumul). Qed.
 
   (** Elimination restriction *)
 
@@ -2260,81 +791,81 @@ Section UnivCF2.
     : config.impl cf1 cf2 ->
       @is_allowed_elimination cf1 φ a s -> @is_allowed_elimination cf2 φ a s.
   Proof using Type.
-    destruct a, s; cbnr; trivial.
-    unfold eq_universe, config.impl, is_true.
+    destruct a, s as [[| |] l]; cbnr; trivial.
+    unfold eq_ulvl, config.impl, is_true.
     do 2 destruct check_univs; cbnr; auto => //.
   Qed.
 
 End UnivCF2.
 
 
-Ltac unfold_univ_rel ::=
+Ltac unfold_univ_rel :=
   unfold is_allowed_elimination, is_lSet, valid_constraints,
-  compare_sort, eq_sort, leq_sort, lt_sort, leq_sort_n, leq_sort_n_, eq_sort_, leqb_sort_n_, eqb_sort_,
-  compare_universe, leq_universe, eq_universe, leq_universe_n in *;
-  destruct check_univs; [unfold_univ_rel0 | trivial].
+  compare_univ, eq_univ, leq_univ, lt_univ, leq_univ_n, leq_univ_n_, eq_univ_, leqb_univ_n_, eqb_univ_,
+  compare_ulvl, leq_ulvl, eq_ulvl, leq_ulvl_n in *;
+  destruct check_univs; [unfold_ulvl_rel0 | trivial].
 
 Tactic Notation "unfold_univ_rel" "eqn" ":"ident(H) :=
   unfold is_allowed_elimination, is_lSet, valid_constraints,
-  compare_sort, eq_sort, leq_sort, lt_sort, leq_sort_n, leq_sort_n_, eq_sort_, leqb_sort_n_, eqb_sort_,
-  compare_universe, leq_universe, eq_universe, leq_universe_n in *;
-  destruct check_univs eqn:H; [unfold_univ_rel0 | trivial].
+  compare_univ, eq_univ, leq_univ, lt_univ, leq_univ_n, leq_univ_n_, eq_univ_, leqb_univ_n_, eqb_univ_,
+  compare_ulvl, leq_ulvl, eq_ulvl, leq_ulvl_n in *;
+  destruct check_univs eqn:H; [unfold_ulvl_rel0 | trivial].
 
 (* Ltac prop_non_prop :=
   match goal with
-  | |- context[ Sort.is_prop ?u || Sort.is_sprop ?u]  =>
-    destruct (Sort.is_prop u || Sort.is_sprop u)
-  | H : context[ Sort.is_prop ?u || Sort.is_sprop ?u] |- _ =>
-    destruct (Sort.is_prop u || Sort.is_sprop u)
+  | |- context[ Universe.is_prop ?u || Universe.is_sprop ?u]  =>
+    destruct (Universe.is_prop u || Universe.is_sprop u)
+  | H : context[ Universe.is_prop ?u || Universe.is_sprop ?u] |- _ =>
+    destruct (Universe.is_prop u || Universe.is_sprop u)
   end. *)
 
 Ltac cong := intuition congruence.
 
 Lemma leq_relevance_eq {cf φ} {s s'} :
-  leq_sort φ s s' -> relevance_of_sort s = relevance_of_sort s'.
+  leq_univ φ s s' -> relevance_of_univ s = relevance_of_univ s'.
 Proof.
-  now destruct s, s'.
+  now destruct s as [[| |] l], s' as [[| |] l'].
 Qed.
 
 Lemma leq_relevance_opt {cf φ} {s s' rel} :
-  leq_sort φ s s' -> isSortRelOpt s rel -> isSortRelOpt s' rel.
+  leq_univ φ s s' -> isUnivRelOpt s rel -> isUnivRelOpt s' rel.
 Proof.
-  now destruct s, s'.
+  now destruct s as [[| |] l], s' as [[| |] l'].
 Qed.
 
 Lemma leq_relevance {cf φ} {s s' rel} :
-  leq_sort φ s s' -> isSortRel s rel -> isSortRel s' rel.
+  leq_univ φ s s' -> isUnivRel s rel -> isUnivRel s' rel.
 Proof.
-  now destruct s, s'.
+    now destruct s as [[| |] l], s' as [[| |] l'].
 Qed.
 
 Lemma geq_relevance {cf φ} {s s' rel} :
-  leq_sort φ s' s -> isSortRel s rel -> isSortRel s' rel.
+  leq_univ φ s' s -> isUnivRel s rel -> isUnivRel s' rel.
 Proof.
-  now destruct s, s'.
+  now destruct s as [[| |] l], s' as [[| |] l'].
 Qed.
 
-Lemma relevance_super s : relevance_of_sort (Sort.super s) = rel_of_Type.
+Lemma relevance_super s : relevance_of_univ (Universe.super s) = rel_of_Type.
 Proof using Type.
-  now destruct s.
+  now destruct s as [[| |] l].
 Qed.
 
-Lemma leq_sort_product_mon {cf} ϕ s1 s1' s2 s2' :
-  leq_sort ϕ s1 s1' ->
-  leq_sort ϕ s2 s2' ->
-  leq_sort ϕ (Sort.sort_of_product s1 s2) (Sort.sort_of_product s1' s2').
+Lemma leq_univ_product_mon {cf} ϕ s1 s1' s2 s2' :
+  leq_univ ϕ s1 s1' ->
+  leq_univ ϕ s2 s2' ->
+  leq_univ ϕ (Universe.univ_of_product s1 s2) (Universe.univ_of_product s1' s2').
 Proof.
-  destruct s2 as [| | u2], s2' as [| | u2']; cbnr; try absurd;
-  destruct s1 as [| | u1], s1' as [| | u1']; cbnr; try absurd; trivial.
-  - intros _ H2; etransitivity; [apply H2 | apply leq_universe_sup_r].
+  destruct s2 as [[| |] u2], s2' as [[| |] u2']; cbnr; try absurd;
+  destruct s1 as [[| |] u1], s1' as [[| |] u1']; cbnr; try absurd; trivial.
+  - intros _ H2; etransitivity; [apply H2 | apply leq_ulvl_sup_r].
   - apply leq_universe_sup_mon.
 Qed.
 
 Lemma impredicative_product {cf} {ϕ l u} :
-  Sort.is_propositional u ->
-  leq_sort ϕ (Sort.sort_of_product l u) u.
+  Universe.is_propositional u ->
+  leq_univ ϕ (Universe.univ_of_product l u) u.
 Proof.
-  destruct u => //; reflexivity.
+  destruct u as [[| |] v] => //; reflexivity.
 Qed.
 
 Section UniverseLemmas.
@@ -2346,17 +877,17 @@ Section UniverseLemmas.
     intro; rewrite !LevelExprSet.union_spec. intuition.
   Qed.
 
-  Lemma sup_idem s : Sort.sup s s = s.
+  Lemma sup_idem s : Universe.sup s s = s.
   Proof using Type.
-    destruct s; cbn; auto.
+    destruct s as [[| |] l]; cbn; auto.
     apply f_equal.
     apply univ_sup_idem.
   Qed.
 
   Lemma sort_of_product_idem s
-    : Sort.sort_of_product s s = s.
+    : Universe.sort_of_product s s = s.
   Proof using Type.
-    unfold Sort.sort_of_product; destruct s; try reflexivity.
+    unfold Universe.sort_of_product; destruct s; try reflexivity.
     apply sup_idem.
   Qed.
 
@@ -2367,23 +898,23 @@ Section UniverseLemmas.
   Qed.
 
   Instance proper_univ_sup_eq_univ φ :
-    Proper (eq_universe φ ==> eq_universe φ ==> eq_universe φ) Universe.sup.
+    Proper (eq_univ φ ==> eq_univ φ ==> eq_univ φ) Universe.sup.
   Proof using Type.
     intros u1 u1' H1 u2 u2' H2.
-    unfold_univ_rel.
+    unfold_ulvl_rel.
     rewrite !val_sup. lia.
   Qed.
 
   Instance proper_sort_sup_eq_sort φ :
-    Proper (eq_sort φ ==> eq_sort φ ==> eq_sort φ) Sort.sup.
+    Proper (eq_sort φ ==> eq_sort φ ==> eq_sort φ) Universe.sup.
   Proof using Type.
     intros [| | u1] [| |u1'] H1 [| |u2] [| |u2'] H2; cbn in *; try absurd; auto.
     now apply proper_univ_sup_eq_univ.
   Qed.
 
   Lemma sort_of_product_twice u s :
-    Sort.sort_of_product u (Sort.sort_of_product u s)
-    = Sort.sort_of_product u s.
+    Universe.sort_of_product u (Universe.sort_of_product u s)
+    = Universe.sort_of_product u s.
   Proof using Type.
     destruct u,s; cbnr.
     now rewrite univ_sup_assoc univ_sup_idem.
@@ -2430,7 +961,7 @@ Section no_prop_leq_type.
 
   Lemma leq_sort_super s s' :
     leq_sort ϕ s s' ->
-    leq_sort ϕ (Sort.super s) (Sort.super s').
+    leq_sort ϕ (Universe.super s) (Universe.super s').
   Proof using Type.
     destruct s as [| | u1], s' as [| | u1']; cbnr; try absurd;
     intros H; unfold_univ_rel;
@@ -2440,7 +971,7 @@ Section no_prop_leq_type.
   Lemma leq_sort_prop_no_prop_sub_type s1 s2 :
     prop_sub_type = false ->
     leq_sort ϕ s1 s2 ->
-    Sort.is_prop s1 -> Sort.is_prop s2.
+    Universe.is_prop s1 -> Universe.is_prop s2.
   Proof using Type.
     intros ps.
     destruct s1; cbn; [ | absurd | absurd].
@@ -2453,7 +984,7 @@ Section no_prop_leq_type.
   Lemma leq_prop_is_propositonal {s1 s2} :
     prop_sub_type = false ->
     leq_sort ϕ s1 s2 ->
-    Sort.is_propositional s1 <-> Sort.is_propositional s2.
+    Universe.is_propositional s1 <-> Universe.is_propositional s2.
   Proof using Type.
     intros ps.
     destruct s1, s2; cbn; try absurd; intros H; split; trivial.
@@ -2509,14 +1040,14 @@ Notation "x @[ u ]" := (subst_instance u x) (at level 3,
 #[global] Instance subst_instance_universe : UnivSubst Universe.t :=
   fun u => map (subst_instance_level_expr u).
 
-#[global] Instance subst_instance_sort : UnivSubst Sort.t :=
+#[global] Instance subst_instance_sort : UnivSubst Universe.t :=
   fun u e => match e with
           | sProp | sSProp => e
           | sType u' => sType (subst_instance u u')
           end.
 
 Lemma subst_instance_to_family s u :
-  Sort.to_family s@[u] = Sort.to_family s.
+  Universe.to_family s@[u] = Universe.to_family s.
 Proof.
   destruct s => //.
 Qed.
@@ -2559,7 +1090,7 @@ Section Closedu.
   Definition closedu_universe (u : Universe.t) :=
     LevelExprSet.for_all closedu_level_expr u.
 
-  Definition closedu_sort (u : Sort.t) :=
+  Definition closedu_sort (u : Universe.t) :=
     match u with
     | sSProp | sProp => true
     | sType l => closedu_universe l
@@ -2681,7 +1212,7 @@ Definition string_of_level (l : Level.t) : string :=
 Definition string_of_level_expr (e : LevelExpr.t) : string :=
   let '(l, n) := e in string_of_level l ^ (if n is 0 then "" else "+" ^ string_of_nat n).
 
-Definition string_of_sort (u : Sort.t) :=
+Definition string_of_sort (u : Universe.t) :=
   match u with
   | sSProp => "SProp"
   | sProp => "Prop"
